<?xml version="1.0"?>


<!DOCTYPE rdf:RDF [
    <!ENTITY bevon "http://rdfs.co/bevon/" >
    <!ENTITY dcterms "http://purl.org/dc/terms/" >
    <!ENTITY adms "http://www.w3.org/ns/adms#" >
    <!ENTITY foaf "http://xmlns.com/foaf/0.1/" >
    <!ENTITY vann "http://purl.org/vocab/vann/" >
    <!ENTITY time "http://www.w3.org/2006/time#" >
    <!ENTITY dbpedia "http://dbpedia.org/ontology/" >
    <!ENTITY yago "http://dbpedia.org/class/yago/" >
    <!ENTITY cc "http://creativecommons.org/ns#" >
    <!ENTITY owl "http://www.w3.org/2002/07/owl#" >
    <!ENTITY beverage "http://rdfs.co/bevon/beverage/" >
    <!ENTITY container "http://rdfs.co/bevon/container/" >
    <!ENTITY gr "http://purl.org/goodrelations/v1#" >
    <!ENTITY xsd "http://www.w3.org/2001/XMLSchema#" >
    <!ENTITY pto "http://www.productontology.org/id/" >
    <!ENTITY whisky "http://purl.org/vocab/whisky/terms/" >
    <!ENTITY skos "http://www.w3.org/2004/02/skos/core#" >
    <!ENTITY food "http://data.lirmm.fr/ontologies/food#" >
    <!ENTITY rdfs "http://www.w3.org/2000/01/rdf-schema#" >
    <!ENTITY rdf "http://www.w3.org/1999/02/22-rdf-syntax-ns#" >
    <!ENTITY status "http://www.w3.org/2003/06/sw-vocab-status/ns#" >
    <!ENTITY wine "http://www.w3.org/TR/2003/PR-owl-guide-20031209/wine#" >
    <!ENTITY fowl "http://www.w3.org/TR/2003/PR-owl-guide-20031209/food#" >
]>


<rdf:RDF xmlns="&bevon;0.7#"
     xml:base="&bevon;0.7"
     xmlns:wine="http://www.w3.org/TR/2003/PR-owl-guide-20031209/wine#"
     xmlns:foaf="http://xmlns.com/foaf/0.1/"
     xmlns:fowl="http://www.w3.org/TR/2003/PR-owl-guide-20031209/food#"
     xmlns:status="http://www.w3.org/2003/06/sw-vocab-status/ns#"
     xmlns:yago="http://dbpedia.org/class/yago/"
     xmlns:vann="http://purl.org/vocab/vann/"
     xmlns:dcterms="http://purl.org/dc/terms/"
     xmlns:adms="http://www.w3.org/ns/adms#"
     xmlns:rdfs="http://www.w3.org/2000/01/rdf-schema#"
     xmlns:time="http://www.w3.org/2006/time#"
     xmlns:beverage="&bevon;beverage/"
     xmlns:container="&bevon;container/"
     xmlns:food="http://data.lirmm.fr/ontologies/food#"
     xmlns:owl="http://www.w3.org/2002/07/owl#"
     xmlns:xsd="http://www.w3.org/2001/XMLSchema#"
     xmlns:dbpedia="http://dbpedia.org/ontology/"
     xmlns:whisky="http://purl.org/vocab/whisky/terms/"
     xmlns:rdf="http://www.w3.org/1999/02/22-rdf-syntax-ns#"
     xmlns:pto="http://www.productontology.org/id/"
     xmlns:bevon="http://rdfs.co/bevon/"
     xmlns:gr="http://purl.org/goodrelations/v1#"
     xmlns:skos="http://www.w3.org/2004/02/skos/core#"
     xmlns:cc="http://creativecommons.org/ns#">
    <owl:Ontology rdf:about="&bevon;0.7">
        <rdfs:comment rdf:datatype="&rdf;XMLLiteral">
    &lt;div&gt;
      The master version of this vocabulary is maintained in &lt;a
      href=&quot;https://github.com/jgkim/bevon&quot;&gt;the GitHub repository&lt;/a&gt; so others
      can contribute edits and improvements.
    &lt;/div&gt;
    </rdfs:comment>
        <dcterms:issued rdf:datatype="&xsd;date">2013-07-04+09:00</dcterms:issued>
        <dcterms:modified rdf:datatype="&xsd;date">2014-03-06+09:00</dcterms:modified>
        <rdfs:comment xml:lang="en">
    Most of the descriptions given here are from Wikipedia or from the websites
    of the related products.
    </rdfs:comment>
        <vann:preferredNamespaceUri>http://rdfs.co/bevon/</vann:preferredNamespaceUri>
        <owl:versionInfo>0.7</owl:versionInfo>
        <dcterms:rights>Copyright © 2013-2014 James G. Kim Some Rights Reserved.</dcterms:rights>
        <vann:preferredNamespacePrefix>bevon</vann:preferredNamespacePrefix>
        <dcterms:identifier>http://rdfs.co/bevon/0.7</dcterms:identifier>
        <cc:license rdf:resource="http://creativecommons.org/licenses/by/4.0/"/>
        <dcterms:creator rdf:resource="http://jayg.me/"/>
        <dcterms:type rdf:resource="http://purl.org/adms/assettype/Ontology"/>
        <adms:status rdf:resource="http://purl.org/adms/status/UnderDevelopment"/>
        <dcterms:isVersionOf rdf:resource="http://rdfs.co/bevon/"/>
        <vann:termGroup rdf:resource="&bevon;BeerGroup"/>
        <vann:termGroup rdf:resource="&bevon;CocktailGroup"/>
        <vann:termGroup rdf:resource="&bevon;ContainerGroup"/>
        <vann:termGroup rdf:resource="&bevon;CoreGroup"/>
        <vann:termGroup rdf:resource="&bevon;RelationGroup"/>
        <vann:termGroup rdf:resource="&bevon;WhiskyGroup"/>
        <vann:termGroup rdf:resource="&bevon;WineGroup"/>
        <dcterms:replaces rdf:resource="&bevon;0.6"/>
        <dcterms:hasFormat rdf:resource="&bevon;0.7/html"/>
        <dcterms:hasFormat rdf:resource="&bevon;0.7/rdf"/>
        <dcterms:hasFormat rdf:resource="&bevon;0.7/ttl"/>
        <rdfs:seeAlso rdf:resource="https://github.com/jgkim/bevon"/>
        <skos:historyNote>
            <rdf:Description/>
        </skos:historyNote>
        <skos:historyNote>
            <rdf:Description/>
        </skos:historyNote>
        <vann:example>
            <rdf:Description/>
        </vann:example>
        <skos:changeNote>
            <rdf:Description/>
        </skos:changeNote>
        <skos:changeNote>
            <rdf:Description/>
        </skos:changeNote>
        <vann:example>
            <rdf:Description/>
        </vann:example>
        <skos:changeNote>
            <rdf:Description/>
        </skos:changeNote>
        <skos:historyNote>
            <rdf:Description/>
        </skos:historyNote>
    </owl:Ontology>
    


    <!-- 
    ///////////////////////////////////////////////////////////////////////////////////////
    //
    // Annotation properties
    //
    ///////////////////////////////////////////////////////////////////////////////////////
     -->

    


    <!-- http://purl.org/dc/terms/creator -->

    <owl:AnnotationProperty rdf:about="&dcterms;creator"/>
    


    <!-- http://purl.org/dc/terms/format -->

    <owl:AnnotationProperty rdf:about="&dcterms;format"/>
    


    <!-- http://purl.org/dc/terms/issued -->

    <owl:AnnotationProperty rdf:about="&dcterms;issued"/>
    


    <!-- http://purl.org/dc/terms/modified -->

    <owl:AnnotationProperty rdf:about="&dcterms;modified"/>
    


    <!-- http://purl.org/vocab/whisky/terms/abv -->

    <owl:AnnotationProperty rdf:about="&whisky;abv">
        <rdfs:subPropertyOf rdf:resource="&bevon;abv"/>
    </owl:AnnotationProperty>
    


    <!-- http://purl.org/vocab/whisky/terms/distillery -->

    <owl:AnnotationProperty rdf:about="&whisky;distillery">
        <rdfs:subPropertyOf rdf:resource="&bevon;distillery"/>
    </owl:AnnotationProperty>
    


    <!-- http://purl.org/vocab/whisky/terms/owner -->

    <owl:AnnotationProperty rdf:about="&whisky;owner"/>
    


    <!-- http://purl.org/vocab/whisky/terms/region -->

    <owl:AnnotationProperty rdf:about="&whisky;region"/>
    


    <!-- http://purl.org/vocab/whisky/terms/waterSource -->

    <owl:AnnotationProperty rdf:about="&whisky;waterSource"/>
    


    <!-- http://rdfs.co/bevon/abv -->

    <rdf:Description rdf:about="&bevon;abv">
        <dcterms:issued rdf:datatype="&xsd;date">2013-07-04+09:00</dcterms:issued>
        <dcterms:modified rdf:datatype="&xsd;date">2014-03-01+09:00</dcterms:modified>
        <skos:definition xml:lang="en">
    ABV (Alcohol by Volume) is a standard measure of how much alcohol is
    contained in the drink.
    </skos:definition>
        <skos:prefLabel xml:lang="en">ABV</skos:prefLabel>
        <skos:altLabel xml:lang="en">alcohol by volume</skos:altLabel>
        <status:term_status xml:lang="en">testing</status:term_status>
        <skos:prefLabel xml:lang="ko">알코올 도수</skos:prefLabel>
        <rdfs:seeAlso rdf:resource="http://en.wikipedia.org/wiki/Alcohol_by_volume"/>
        <rdfs:isDefinedBy rdf:resource="http://rdfs.co/bevon/"/>
    </rdf:Description>
    


    <!-- http://rdfs.co/bevon/distillery -->

    <rdf:Description rdf:about="&bevon;distillery">
        <dcterms:issued rdf:datatype="&xsd;date">2013-07-04+09:00</dcterms:issued>
        <dcterms:modified rdf:datatype="&xsd;date">2014-03-01+09:00</dcterms:modified>
        <skos:definition xml:lang="en">
    This property relates a distilled beverage to its distillery.
    </skos:definition>
        <skos:prefLabel xml:lang="en">Distillery</skos:prefLabel>
        <status:term_status xml:lang="en">unstable</status:term_status>
        <skos:prefLabel xml:lang="ko">증류소</skos:prefLabel>
        <rdfs:seeAlso rdf:resource="http://en.wikipedia.org/wiki/Distillation"/>
        <rdfs:isDefinedBy rdf:resource="http://rdfs.co/bevon/"/>
    </rdf:Description>
    


    <!-- http://www.w3.org/2000/01/rdf-schema#commercial -->

    <owl:AnnotationProperty rdf:about="&rdfs;commercial"/>
    


    <!-- http://www.w3.org/2003/06/sw-vocab-status/ns#term_status -->

    <owl:AnnotationProperty rdf:about="&status;term_status"/>
    


    <!-- http://www.w3.org/2004/02/skos/core#altLabel -->

    <owl:AnnotationProperty rdf:about="&skos;altLabel"/>
    


    <!-- http://www.w3.org/2004/02/skos/core#definition -->

    <owl:AnnotationProperty rdf:about="&skos;definition"/>
    


    <!-- http://www.w3.org/2004/02/skos/core#historyNote -->

    <owl:AnnotationProperty rdf:about="&skos;historyNote"/>
    


    <!-- http://www.w3.org/2004/02/skos/core#prefLabel -->

    <owl:AnnotationProperty rdf:about="&skos;prefLabel"/>
    


    <!-- http://xmlns.com/foaf/0.1/homepage -->

    <owl:AnnotationProperty rdf:about="&foaf;homepage"/>
    


    <!-- http://xmlns.com/foaf/0.1/mbox_sha1sum -->

    <owl:AnnotationProperty rdf:about="&foaf;mbox_sha1sum"/>
    


    <!-- 
    ///////////////////////////////////////////////////////////////////////////////////////
    //
    // Datatypes
    //
    ///////////////////////////////////////////////////////////////////////////////////////
     -->

    


    <!-- http://www.w3.org/2001/XMLSchema#date -->

    <rdfs:Datatype rdf:about="&xsd;date"/>
    


    <!-- http://www.w3.org/2001/XMLSchema#gYear -->

    <rdfs:Datatype rdf:about="&xsd;gYear"/>
    


    <!-- 
    ///////////////////////////////////////////////////////////////////////////////////////
    //
    // Object Properties
    //
    ///////////////////////////////////////////////////////////////////////////////////////
     -->

    


    <!-- http://data.lirmm.fr/ontologies/food#containsIngredient -->

    <owl:ObjectProperty rdf:about="&food;containsIngredient"/>
    


    <!-- http://data.lirmm.fr/ontologies/food#food -->

    <owl:ObjectProperty rdf:about="&food;food"/>
    


    <!-- http://dbpedia.org/ontology/variantOf -->

    <owl:ObjectProperty rdf:about="&dbpedia;variantOf"/>
    


    <!-- http://purl.org/goodrelations/v1#hasManufacturer -->

    <owl:ObjectProperty rdf:about="&gr;hasManufacturer"/>
    


    <!-- http://purl.org/goodrelations/v1#isSimilarTo -->

    <owl:ObjectProperty rdf:about="&gr;isSimilarTo"/>
    


    <!-- http://purl.org/goodrelations/v1#isVariantOf -->

    <owl:ObjectProperty rdf:about="&gr;isVariantOf"/>
    


    <!-- http://rdfs.co/bevon/aging -->

    <owl:ObjectProperty rdf:about="&bevon;aging">
        <dcterms:issued rdf:datatype="&xsd;date">2013-07-04+09:00</dcterms:issued>
        <dcterms:modified rdf:datatype="&xsd;date">2014-03-01+09:00</dcterms:modified>
        <skos:definition xml:lang="en">
    This property specifies how the beverage has been aged.
    </skos:definition>
        <skos:prefLabel xml:lang="en">aging</skos:prefLabel>
        <status:term_status xml:lang="en">unstable</status:term_status>
        <skos:prefLabel xml:lang="ko">숙성</skos:prefLabel>
        <rdfs:isDefinedBy rdf:resource="http://rdfs.co/bevon/"/>
        <rdfs:range rdf:resource="&bevon;Aging"/>
        <rdfs:domain rdf:resource="&bevon;AlcoholicBeverage"/>
    </owl:ObjectProperty>
    


    <!-- http://rdfs.co/bevon/brewery -->

    <owl:ObjectProperty rdf:about="&bevon;brewery">
        <dcterms:issued rdf:datatype="&xsd;date">2013-07-04+09:00</dcterms:issued>
        <dcterms:modified rdf:datatype="&xsd;date">2014-03-01+09:00</dcterms:modified>
        <skos:definition xml:lang="en">
    This property relates a beer to its brewery.
    </skos:definition>
        <skos:prefLabel xml:lang="en">Brewery</skos:prefLabel>
        <status:term_status xml:lang="en">unstable</status:term_status>
        <skos:prefLabel xml:lang="ko">양조장</skos:prefLabel>
        <rdfs:seeAlso rdf:resource="http://en.wikipedia.org/wiki/Brewery"/>
        <rdfs:isDefinedBy rdf:resource="http://rdfs.co/bevon/"/>
        <rdfs:domain rdf:resource="&bevon;Beer"/>
        <rdfs:range rdf:resource="&bevon;Brewery"/>
    </owl:ObjectProperty>
    


    <!-- http://rdfs.co/bevon/color -->

    <owl:ObjectProperty rdf:about="&bevon;color">
        <dcterms:issued rdf:datatype="&xsd;date">2013-07-04+09:00</dcterms:issued>
        <dcterms:modified rdf:datatype="&xsd;date">2014-03-01+09:00</dcterms:modified>
        <skos:definition xml:lang="en">
    This property specifies the color of the beverage.
    </skos:definition>
        <skos:prefLabel xml:lang="en">color</skos:prefLabel>
        <status:term_status xml:lang="en">unstable</status:term_status>
        <skos:prefLabel xml:lang="ko">색상</skos:prefLabel>
        <rdfs:range rdf:resource="&dbpedia;Colour"/>
        <rdfs:isDefinedBy rdf:resource="http://rdfs.co/bevon/"/>
        <rdfs:domain rdf:resource="&bevon;Beverage"/>
    </owl:ObjectProperty>
    


    <!-- http://rdfs.co/bevon/container -->

    <owl:ObjectProperty rdf:about="&bevon;container">
        <dcterms:issued rdf:datatype="&xsd;date">2013-07-04+09:00</dcterms:issued>
        <dcterms:modified rdf:datatype="&xsd;date">2014-03-01+09:00</dcterms:modified>
        <skos:definition xml:lang="en">
    This property can be used to indicate that the beverage is available in a
    type of container.
    </skos:definition>
        <skos:prefLabel xml:lang="en">container</skos:prefLabel>
        <status:term_status xml:lang="en">unstable</status:term_status>
        <skos:prefLabel xml:lang="ko">용기</skos:prefLabel>
        <rdfs:isDefinedBy rdf:resource="http://rdfs.co/bevon/"/>
        <rdfs:domain rdf:resource="&bevon;Beverage"/>
        <rdfs:range rdf:resource="&bevon;Container"/>
    </owl:ObjectProperty>
    


    <!-- http://rdfs.co/bevon/distillery -->

    <owl:ObjectProperty rdf:about="&bevon;distillery">
        <dcterms:issued rdf:datatype="&xsd;date">2013-07-04+09:00</dcterms:issued>
        <dcterms:modified rdf:datatype="&xsd;date">2014-03-01+09:00</dcterms:modified>
        <skos:definition xml:lang="en">
    This property relates a distilled beverage to its distillery.
    </skos:definition>
        <skos:prefLabel xml:lang="en">Distillery</skos:prefLabel>
        <status:term_status xml:lang="en">unstable</status:term_status>
        <skos:prefLabel xml:lang="ko">증류소</skos:prefLabel>
        <rdfs:seeAlso rdf:resource="http://en.wikipedia.org/wiki/Distillation"/>
        <rdfs:isDefinedBy rdf:resource="http://rdfs.co/bevon/"/>
        <rdfs:domain rdf:resource="&bevon;DistilledBeverage"/>
        <rdfs:range rdf:resource="&bevon;Distillery"/>
    </owl:ObjectProperty>
    


    <!-- http://rdfs.co/bevon/duration -->

    <owl:ObjectProperty rdf:about="&bevon;duration">
        <dcterms:issued rdf:datatype="&xsd;date">2013-07-04+09:00</dcterms:issued>
        <dcterms:modified rdf:datatype="&xsd;date">2014-03-01+09:00</dcterms:modified>
        <skos:definition xml:lang="en">
    This property describes how long the beverage was aged in the cask.
    </skos:definition>
        <skos:prefLabel xml:lang="en">duration</skos:prefLabel>
        <status:term_status xml:lang="en">unstable</status:term_status>
        <skos:prefLabel xml:lang="ko">기간</skos:prefLabel>
        <rdfs:isDefinedBy rdf:resource="http://rdfs.co/bevon/"/>
        <rdfs:domain rdf:resource="&bevon;Aging"/>
        <rdfs:range rdf:resource="&time;DurationDescription"/>
        <rdfs:subPropertyOf rdf:resource="&time;hasDurationDescription"/>
    </owl:ObjectProperty>
    


    <!-- http://rdfs.co/bevon/fermentation_base -->

    <owl:ObjectProperty rdf:about="&bevon;fermentation_base">
        <dcterms:issued rdf:datatype="&xsd;date">2013-07-04+09:00</dcterms:issued>
        <dcterms:modified rdf:datatype="&xsd;date">2014-03-01+09:00</dcterms:modified>
        <skos:definition xml:lang="en">
    This property indicates which fermentation base is used to make the
    alcoholic beverage.
    </skos:definition>
        <skos:prefLabel xml:lang="en">fermentation base</skos:prefLabel>
        <status:term_status xml:lang="en">unstable</status:term_status>
        <skos:prefLabel xml:lang="ko">발효 주재료</skos:prefLabel>
        <rdfs:isDefinedBy rdf:resource="http://rdfs.co/bevon/"/>
        <rdfs:domain rdf:resource="&bevon;AlcoholicBeverage"/>
        <rdfs:range rdf:resource="&bevon;FermentationBase"/>
    </owl:ObjectProperty>
    


    <!-- http://rdfs.co/bevon/food -->

    <owl:ObjectProperty rdf:about="&bevon;food">
        <dcterms:issued rdf:datatype="&xsd;date">2013-07-04+09:00</dcterms:issued>
        <dcterms:modified rdf:datatype="&xsd;date">2014-03-01+09:00</dcterms:modified>
        <skos:definition xml:lang="en">
    This property describes food that is an ingredient of a mixed drink.
    </skos:definition>
        <skos:prefLabel xml:lang="en">food</skos:prefLabel>
        <status:term_status xml:lang="en">unstable</status:term_status>
        <skos:prefLabel xml:lang="ko">음식</skos:prefLabel>
        <rdfs:range rdf:resource="&food;Food"/>
        <rdfs:domain rdf:resource="&food;Ingredient"/>
        <rdfs:subPropertyOf rdf:resource="&food;food"/>
        <rdfs:isDefinedBy rdf:resource="http://rdfs.co/bevon/"/>
    </owl:ObjectProperty>
    


    <!-- http://rdfs.co/bevon/ingredient -->

    <owl:ObjectProperty rdf:about="&bevon;ingredient">
        <dcterms:issued rdf:datatype="&xsd;date">2013-07-04+09:00</dcterms:issued>
        <dcterms:modified rdf:datatype="&xsd;date">2014-03-01+09:00</dcterms:modified>
        <skos:definition xml:lang="en">
    This property specifies an ingredient of the mixed drink.
    </skos:definition>
        <skos:prefLabel xml:lang="en">ingredient</skos:prefLabel>
        <status:term_status xml:lang="en">unstable</status:term_status>
        <skos:prefLabel xml:lang="ko">재료</skos:prefLabel>
        <rdfs:range rdf:resource="&food;Ingredient"/>
        <rdfs:subPropertyOf rdf:resource="&food;containsIngredient"/>
        <rdfs:isDefinedBy rdf:resource="http://rdfs.co/bevon/"/>
        <rdfs:domain rdf:resource="&bevon;MixedDrink"/>
    </owl:ObjectProperty>
    


    <!-- http://rdfs.co/bevon/manufacturer -->

    <owl:ObjectProperty rdf:about="&bevon;manufacturer">
        <dcterms:issued rdf:datatype="&xsd;date">2013-07-04+09:00</dcterms:issued>
        <dcterms:modified rdf:datatype="&xsd;date">2014-03-01+09:00</dcterms:modified>
        <skos:definition xml:lang="en">
    This property specifies the manufacturer of the beverage.
    </skos:definition>
        <skos:prefLabel xml:lang="en">manufacturer</skos:prefLabel>
        <status:term_status xml:lang="en">unstable</status:term_status>
        <skos:prefLabel xml:lang="ko">제조사</skos:prefLabel>
        <rdfs:subPropertyOf rdf:resource="&gr;hasManufacturer"/>
        <rdfs:isDefinedBy rdf:resource="http://rdfs.co/bevon/"/>
        <rdfs:domain rdf:resource="&bevon;Beverage"/>
        <rdfs:range rdf:resource="&foaf;Agent"/>
    </owl:ObjectProperty>
    


    <!-- http://rdfs.co/bevon/material -->

    <owl:ObjectProperty rdf:about="&bevon;material">
        <dcterms:issued rdf:datatype="&xsd;date">2013-07-04+09:00</dcterms:issued>
        <dcterms:modified rdf:datatype="&xsd;date">2014-03-01+09:00</dcterms:modified>
        <skos:definition xml:lang="en">
    This property specifies what the aging cask was made of.
    </skos:definition>
        <skos:prefLabel xml:lang="en">material</skos:prefLabel>
        <status:term_status xml:lang="en">unstable</status:term_status>
        <skos:prefLabel xml:lang="ko">소재</skos:prefLabel>
        <rdfs:isDefinedBy rdf:resource="http://rdfs.co/bevon/"/>
        <rdfs:domain rdf:resource="&bevon;Aging"/>
    </owl:ObjectProperty>
    


    <!-- http://rdfs.co/bevon/non_alcoholic_version -->

    <owl:ObjectProperty rdf:about="&bevon;non_alcoholic_version">
        <dcterms:issued rdf:datatype="&xsd;date">2013-07-04+09:00</dcterms:issued>
        <dcterms:modified rdf:datatype="&xsd;date">2014-03-01+09:00</dcterms:modified>
        <skos:definition xml:lang="en">
    Some alcoholic beverages have non-alcoholic versions, such as non-alcoholic
    beer (&quot;near beer&quot;) and cocktails (&quot;mocktails&quot;).
    </skos:definition>
        <skos:prefLabel xml:lang="en">non-alcoholic version</skos:prefLabel>
        <status:term_status xml:lang="en">unstable</status:term_status>
        <skos:prefLabel xml:lang="ko">비알코올 버전</skos:prefLabel>
        <rdfs:isDefinedBy rdf:resource="http://rdfs.co/bevon/"/>
        <rdfs:domain rdf:resource="&bevon;AlcoholicBeverage"/>
        <rdfs:range rdf:resource="&bevon;NonAlcoholicBeverage"/>
        <rdfs:subPropertyOf rdf:resource="&bevon;related"/>
    </owl:ObjectProperty>
    


    <!-- http://rdfs.co/bevon/origin -->

    <owl:ObjectProperty rdf:about="&bevon;origin">
        <dcterms:issued rdf:datatype="&xsd;date">2013-07-04+09:00</dcterms:issued>
        <dcterms:modified rdf:datatype="&xsd;date">2014-03-01+09:00</dcterms:modified>
        <skos:definition xml:lang="en">
    This property indicates the place where the beverage was first invented.
    </skos:definition>
        <skos:prefLabel xml:lang="en">origin</skos:prefLabel>
        <status:term_status xml:lang="en">unstable</status:term_status>
        <skos:prefLabel xml:lang="ko">원산지</skos:prefLabel>
        <rdfs:range rdf:resource="&dbpedia;Place"/>
        <rdfs:isDefinedBy rdf:resource="http://rdfs.co/bevon/"/>
        <rdfs:domain rdf:resource="&bevon;Beverage"/>
    </owl:ObjectProperty>
    


    <!-- http://rdfs.co/bevon/previous_content -->

    <owl:ObjectProperty rdf:about="&bevon;previous_content">
        <dcterms:issued rdf:datatype="&xsd;date">2013-07-04+09:00</dcterms:issued>
        <dcterms:modified rdf:datatype="&xsd;date">2014-03-01+09:00</dcterms:modified>
        <skos:definition xml:lang="en">
    This property specifies what as in the cask before the aging.
    </skos:definition>
        <skos:prefLabel xml:lang="en">previous content</skos:prefLabel>
        <status:term_status xml:lang="en">unstable</status:term_status>
        <skos:prefLabel xml:lang="ko">이전 내용물</skos:prefLabel>
        <rdfs:isDefinedBy rdf:resource="http://rdfs.co/bevon/"/>
        <rdfs:domain rdf:resource="&bevon;Aging"/>
        <rdfs:range rdf:resource="&fowl;PotableLiquid"/>
    </owl:ObjectProperty>
    


    <!-- http://rdfs.co/bevon/quantity -->

    <owl:ObjectProperty rdf:about="&bevon;quantity">
        <dcterms:issued rdf:datatype="&xsd;date">2013-07-04+09:00</dcterms:issued>
        <dcterms:modified rdf:datatype="&xsd;date">2014-03-01+09:00</dcterms:modified>
        <skos:definition xml:lang="en">
    This property specifies the quantity of the ingredient with a type
    in the UN/CEFACT Common Code.
    </skos:definition>
        <skos:prefLabel xml:lang="en">quantity</skos:prefLabel>
        <status:term_status xml:lang="en">unstable</status:term_status>
        <skos:prefLabel xml:lang="ko">양</skos:prefLabel>
        <rdfs:domain rdf:resource="&food;Ingredient"/>
        <rdfs:range rdf:resource="&gr;QuantitativeValue"/>
        <rdfs:isDefinedBy rdf:resource="http://rdfs.co/bevon/"/>
    </owl:ObjectProperty>
    


    <!-- http://rdfs.co/bevon/related -->

    <owl:ObjectProperty rdf:about="&bevon;related">
        <dcterms:issued rdf:datatype="&xsd;date">2013-07-04+09:00</dcterms:issued>
        <dcterms:modified rdf:datatype="&xsd;date">2014-03-01+09:00</dcterms:modified>
        <skos:definition xml:lang="en">
    This property states that a beverage is related to another beverage.
    </skos:definition>
        <skos:prefLabel xml:lang="en">related</skos:prefLabel>
        <status:term_status xml:lang="en">unstable</status:term_status>
        <skos:prefLabel xml:lang="ko">연관</skos:prefLabel>
        <rdfs:isDefinedBy rdf:resource="http://rdfs.co/bevon/"/>
        <rdfs:domain rdf:resource="&bevon;Beverage"/>
        <rdfs:range rdf:resource="&bevon;Beverage"/>
    </owl:ObjectProperty>
    


    <!-- http://rdfs.co/bevon/similar -->

    <owl:ObjectProperty rdf:about="&bevon;similar">
        <rdf:type rdf:resource="&owl;SymmetricProperty"/>
        <dcterms:issued rdf:datatype="&xsd;date">2013-07-04+09:00</dcterms:issued>
        <dcterms:modified rdf:datatype="&xsd;date">2014-03-01+09:00</dcterms:modified>
        <skos:definition xml:lang="en">
    This property states that a beverage is similar to another beverage.
    </skos:definition>
        <skos:prefLabel xml:lang="en">similar</skos:prefLabel>
        <status:term_status xml:lang="en">unstable</status:term_status>
        <skos:prefLabel xml:lang="ko">유사</skos:prefLabel>
        <rdfs:subPropertyOf rdf:resource="&gr;isSimilarTo"/>
        <rdfs:isDefinedBy rdf:resource="http://rdfs.co/bevon/"/>
        <rdfs:range rdf:resource="&bevon;Beverage"/>
        <rdfs:domain rdf:resource="&bevon;Beverage"/>
        <rdfs:subPropertyOf rdf:resource="&bevon;related"/>
    </owl:ObjectProperty>
    


    <!-- http://rdfs.co/bevon/variant -->

    <owl:ObjectProperty rdf:about="&bevon;variant">
        <dcterms:issued rdf:datatype="&xsd;date">2013-07-04+09:00</dcterms:issued>
        <dcterms:modified rdf:datatype="&xsd;date">2014-03-01+09:00</dcterms:modified>
        <skos:definition xml:lang="en">
    This property states that a beverage has a variant.
    </skos:definition>
        <status:term_status xml:lang="en">unstable</status:term_status>
        <skos:prefLabel xml:lang="en">variant</skos:prefLabel>
        <skos:prefLabel xml:lang="ko">변형</skos:prefLabel>
        <rdfs:isDefinedBy rdf:resource="http://rdfs.co/bevon/"/>
        <rdfs:range rdf:resource="&bevon;Beverage"/>
        <rdfs:domain rdf:resource="&bevon;Beverage"/>
        <rdfs:subPropertyOf rdf:resource="&bevon;related"/>
    </owl:ObjectProperty>
    


    <!-- http://rdfs.co/bevon/variantOf -->

    <owl:ObjectProperty rdf:about="&bevon;variantOf">
        <dcterms:issued rdf:datatype="&xsd;date">2013-07-04+09:00</dcterms:issued>
        <dcterms:modified rdf:datatype="&xsd;date">2014-03-01+09:00</dcterms:modified>
        <skos:definition xml:lang="en">
    This property states that a beverage is a variant of another beverage.
    </skos:definition>
        <status:term_status xml:lang="en">unstable</status:term_status>
        <skos:prefLabel xml:lang="en">variant of</skos:prefLabel>
        <skos:prefLabel xml:lang="ko">바탕</skos:prefLabel>
        <rdfs:subPropertyOf rdf:resource="&dbpedia;variantOf"/>
        <rdfs:subPropertyOf rdf:resource="&gr;isVariantOf"/>
        <rdfs:isDefinedBy rdf:resource="http://rdfs.co/bevon/"/>
        <rdfs:domain rdf:resource="&bevon;Beverage"/>
        <rdfs:range rdf:resource="&bevon;Beverage"/>
        <rdfs:subPropertyOf rdf:resource="&bevon;related"/>
        <owl:inverseOf rdf:resource="&bevon;variant"/>
    </owl:ObjectProperty>
    


    <!-- http://rdfs.co/bevon/volume -->

    <owl:ObjectProperty rdf:about="&bevon;volume">
        <dcterms:issued rdf:datatype="&xsd;date">2013-07-04+09:00</dcterms:issued>
        <dcterms:modified rdf:datatype="&xsd;date">2014-03-01+09:00</dcterms:modified>
        <skos:definition xml:lang="en">
    This property specifies the volume of the container.
    </skos:definition>
        <status:term_status xml:lang="en">unstable</status:term_status>
        <skos:prefLabel xml:lang="en">volume</skos:prefLabel>
        <skos:prefLabel xml:lang="ko">용량</skos:prefLabel>
        <rdfs:range rdf:resource="&gr;QuantitativeValue"/>
        <rdfs:isDefinedBy rdf:resource="http://rdfs.co/bevon/"/>
        <rdfs:domain rdf:resource="&bevon;Container"/>
    </owl:ObjectProperty>
    


    <!-- http://www.w3.org/2006/time#hasDurationDescription -->

    <owl:ObjectProperty rdf:about="&time;hasDurationDescription"/>
    


    <!-- 
    ///////////////////////////////////////////////////////////////////////////////////////
    //
    // Data properties
    //
    ///////////////////////////////////////////////////////////////////////////////////////
     -->

    


    <!-- http://purl.org/dc/terms/description -->

    <owl:DatatypeProperty rdf:about="&dcterms;description"/>
    


    <!-- http://purl.org/dc/terms/title -->

    <owl:DatatypeProperty rdf:about="&dcterms;title"/>
    


    <!-- http://purl.org/goodrelations/v1#description -->

    <owl:DatatypeProperty rdf:about="&gr;description"/>
    


    <!-- http://purl.org/goodrelations/v1#name -->

    <owl:DatatypeProperty rdf:about="&gr;name"/>
    


    <!-- http://rdfs.co/bevon/abv -->

    <owl:DatatypeProperty rdf:about="&bevon;abv">
        <dcterms:issued rdf:datatype="&xsd;date">2013-07-04+09:00</dcterms:issued>
        <dcterms:modified rdf:datatype="&xsd;date">2014-03-01+09:00</dcterms:modified>
        <skos:definition xml:lang="en">
    ABV (Alcohol by Volume) is a standard measure of how much alcohol is
    contained in the drink.
    </skos:definition>
        <skos:prefLabel xml:lang="en">ABV</skos:prefLabel>
        <skos:altLabel xml:lang="en">alcohol by volume</skos:altLabel>
        <status:term_status xml:lang="en">testing</status:term_status>
        <skos:prefLabel xml:lang="ko">알코올 도수</skos:prefLabel>
        <rdfs:seeAlso rdf:resource="http://en.wikipedia.org/wiki/Alcohol_by_volume"/>
        <rdfs:isDefinedBy rdf:resource="http://rdfs.co/bevon/"/>
        <rdfs:domain rdf:resource="&bevon;Beverage"/>
        <rdfs:range rdf:resource="&xsd;decimal"/>
    </owl:DatatypeProperty>
    


    <!-- http://rdfs.co/bevon/color -->

    <owl:DatatypeProperty rdf:about="&bevon;color">
        <dcterms:issued rdf:datatype="&xsd;date">2013-07-04+09:00</dcterms:issued>
        <dcterms:modified rdf:datatype="&xsd;date">2014-03-01+09:00</dcterms:modified>
        <skos:definition xml:lang="en">
    This property specifies the color of the beverage.
    </skos:definition>
        <skos:prefLabel xml:lang="en">color</skos:prefLabel>
        <status:term_status xml:lang="en">unstable</status:term_status>
        <skos:prefLabel xml:lang="ko">색상</skos:prefLabel>
        <rdfs:isDefinedBy rdf:resource="http://rdfs.co/bevon/"/>
    </owl:DatatypeProperty>
    


    <!-- http://rdfs.co/bevon/description -->

    <owl:DatatypeProperty rdf:about="&bevon;description">
        <dcterms:issued rdf:datatype="&xsd;date">2013-07-04+09:00</dcterms:issued>
        <dcterms:modified rdf:datatype="&xsd;date">2014-03-01+09:00</dcterms:modified>
        <skos:definition xml:lang="en">
    This property specifies the short text description of the beverage.
    </skos:definition>
        <skos:prefLabel xml:lang="en">description</skos:prefLabel>
        <status:term_status xml:lang="en">testing</status:term_status>
        <skos:prefLabel xml:lang="ko">설명</skos:prefLabel>
        <rdfs:subPropertyOf rdf:resource="&dcterms;description"/>
        <rdfs:subPropertyOf rdf:resource="&gr;description"/>
        <rdfs:isDefinedBy rdf:resource="http://rdfs.co/bevon/"/>
        <rdfs:domain rdf:resource="&bevon;Beverage"/>
        <rdfs:range rdf:resource="&xsd;string"/>
    </owl:DatatypeProperty>
    


    <!-- http://rdfs.co/bevon/ibu -->

    <owl:DatatypeProperty rdf:about="&bevon;ibu">
        <dcterms:issued rdf:datatype="&xsd;date">2013-07-04+09:00</dcterms:issued>
        <dcterms:modified rdf:datatype="&xsd;date">2014-03-01+09:00</dcterms:modified>
        <skos:definition xml:lang="en">
    The International Bittering Units scale, or simply IBU scale, provides a
    measure of the bitterness of beer, which is provided by the hops used
    during brewing.
    </skos:definition>
        <skos:prefLabel xml:lang="en">IBU scale</skos:prefLabel>
        <skos:altLabel xml:lang="en">International Bitterness Unit scale</skos:altLabel>
        <status:term_status xml:lang="en">unstable</status:term_status>
        <skos:prefLabel xml:lang="ko">IBU 척도</skos:prefLabel>
        <rdfs:seeAlso rdf:resource="http://en.wikipedia.org/wiki/International_Bitterness_Units_scale"/>
        <rdfs:isDefinedBy rdf:resource="http://rdfs.co/bevon/"/>
        <rdfs:domain rdf:resource="&bevon;Beer"/>
        <rdfs:range rdf:resource="&xsd;nonNegativeInteger"/>
    </owl:DatatypeProperty>
    


    <!-- http://rdfs.co/bevon/launch -->

    <owl:DatatypeProperty rdf:about="&bevon;launch">
        <dcterms:issued rdf:datatype="&xsd;date">2013-07-04+09:00</dcterms:issued>
        <dcterms:modified rdf:datatype="&xsd;date">2014-03-01+09:00</dcterms:modified>
        <skos:definition xml:lang="en">
    This property specifies the year when the beverage was first introduced to
    the market.
    </skos:definition>
        <skos:prefLabel xml:lang="en">launch</skos:prefLabel>
        <status:term_status xml:lang="en">unstable</status:term_status>
        <skos:prefLabel xml:lang="ko">출시년도</skos:prefLabel>
        <rdfs:isDefinedBy rdf:resource="http://rdfs.co/bevon/"/>
        <rdfs:domain rdf:resource="&bevon;Beverage"/>
        <rdfs:range rdf:resource="&xsd;gYear"/>
    </owl:DatatypeProperty>
    


    <!-- http://rdfs.co/bevon/name -->

    <owl:DatatypeProperty rdf:about="&bevon;name">
        <dcterms:issued rdf:datatype="&xsd;date">2013-07-04+09:00</dcterms:issued>
        <dcterms:modified rdf:datatype="&xsd;date">2014-03-01+09:00</dcterms:modified>
        <skos:definition xml:lang="en">
    This property indicates the name of the beverage.
    </skos:definition>
        <skos:prefLabel xml:lang="en">name</skos:prefLabel>
        <status:term_status xml:lang="en">testing</status:term_status>
        <skos:prefLabel xml:lang="ko">이름</skos:prefLabel>
        <rdfs:subPropertyOf rdf:resource="&dcterms;title"/>
        <rdfs:subPropertyOf rdf:resource="&gr;name"/>
        <rdfs:isDefinedBy rdf:resource="http://rdfs.co/bevon/"/>
        <rdfs:domain rdf:resource="&bevon;Beverage"/>
        <rdfs:range rdf:resource="&xsd;string"/>
        <rdfs:subPropertyOf rdf:resource="&foaf;name"/>
    </owl:DatatypeProperty>
    


    <!-- http://rdfs.co/bevon/proof -->

    <owl:DatatypeProperty rdf:about="&bevon;proof">
        <dcterms:issued rdf:datatype="&xsd;date">2013-07-04+09:00</dcterms:issued>
        <dcterms:modified rdf:datatype="&xsd;date">2014-03-01+09:00</dcterms:modified>
        <skos:definition xml:lang="en">
    Alcohol proof is a measure of how much alcohol (ethanol) is contained in an
    alcoholic beverage.
    </skos:definition>
        <rdfs:comment xml:lang="en">
    The term was originally used in the United Kingdom and was defined as 7/4
    times the alcohol by volume (ABV). The UK now uses the ABV standard instead
    of alcohol proof. In the United States, alcoholic proof is defined as twice
    the percentage of ABV.
    </rdfs:comment>
        <skos:altLabel xml:lang="en">alcohol proof</skos:altLabel>
        <skos:prefLabel xml:lang="en">proof</skos:prefLabel>
        <status:term_status xml:lang="en">unstable</status:term_status>
        <skos:prefLabel xml:lang="ko">프루프</skos:prefLabel>
        <rdfs:seeAlso rdf:resource="http://en.wikipedia.org/wiki/Alcohol_proof"/>
        <rdfs:isDefinedBy rdf:resource="http://rdfs.co/bevon/"/>
        <rdfs:domain rdf:resource="&bevon;Beverage"/>
        <rdfs:range rdf:resource="&xsd;decimal"/>
    </owl:DatatypeProperty>
    


    <!-- http://rdfs.co/bevon/srm -->

    <owl:DatatypeProperty rdf:about="&bevon;srm">
        <dcterms:issued rdf:datatype="&xsd;date">2013-07-04+09:00</dcterms:issued>
        <dcterms:modified rdf:datatype="&xsd;date">2014-03-01+09:00</dcterms:modified>
        <skos:definition xml:lang="en">
    The Standard Reference Method or SRM is one of several systems modern
    brewers use to specify beer color.
    </skos:definition>
        <skos:prefLabel xml:lang="en">SRM</skos:prefLabel>
        <skos:altLabel xml:lang="en">Standard Reference Method</skos:altLabel>
        <status:term_status xml:lang="en">unstable</status:term_status>
        <rdfs:seeAlso rdf:resource="http://en.wikipedia.org/wiki/Standard_Reference_Method"/>
        <rdfs:isDefinedBy rdf:resource="http://rdfs.co/bevon/"/>
        <rdfs:domain rdf:resource="&bevon;Beer"/>
        <rdfs:range rdf:resource="&xsd;nonNegativeInteger"/>
    </owl:DatatypeProperty>
    


    <!-- http://xmlns.com/foaf/0.1/name -->

    <owl:DatatypeProperty rdf:about="&foaf;name"/>
    


    <!-- 
    ///////////////////////////////////////////////////////////////////////////////////////
    //
    // Classes
    //
    ///////////////////////////////////////////////////////////////////////////////////////
     -->

    


    <!-- http://creativecommons.org/ns#Work -->

    <owl:Class rdf:about="&cc;Work"/>
    


    <!-- http://data.lirmm.fr/ontologies/food#Food -->

    <owl:Class rdf:about="&food;Food"/>
    


    <!-- http://data.lirmm.fr/ontologies/food#Ingredient -->

    <owl:Class rdf:about="&food;Ingredient"/>
    


    <!-- http://dbpedia.org/class/yago/Containers -->

    <owl:Class rdf:about="&yago;Containers"/>
    


    <!-- http://dbpedia.org/ontology/Colour -->

    <owl:Class rdf:about="&dbpedia;Colour"/>
    


    <!-- http://dbpedia.org/ontology/Place -->

    <owl:Class rdf:about="&dbpedia;Place"/>
    


    <!-- http://purl.org/dc/terms/IMT -->

    <owl:Class rdf:about="&dcterms;IMT"/>
    


    <!-- http://purl.org/goodrelations/v1#ProductOrServiceModel -->

    <owl:Class rdf:about="&gr;ProductOrServiceModel"/>
    


    <!-- http://purl.org/goodrelations/v1#QuantitativeValue -->

    <owl:Class rdf:about="&gr;QuantitativeValue"/>
    


    <!-- http://purl.org/goodrelations/v1#QuantitativeValueFloat -->

    <owl:Class rdf:about="&gr;QuantitativeValueFloat"/>
    


    <!-- http://purl.org/goodrelations/v1#QuantitativeValueInteger -->

    <owl:Class rdf:about="&gr;QuantitativeValueInteger"/>
    


    <!-- http://purl.org/vocab/whisky/terms/Distillery -->

    <owl:Class rdf:about="&whisky;Distillery">
        <rdfs:subClassOf rdf:resource="&bevon;Distillery"/>
    </owl:Class>
    


    <!-- http://purl.org/vocab/whisky/terms/WaterSource -->

    <owl:Class rdf:about="&whisky;WaterSource"/>
    


    <!-- http://rdfs.co/bevon/Aging -->

    <owl:Class rdf:about="&bevon;Aging">
        <dcterms:issued rdf:datatype="&xsd;date">2013-07-04+09:00</dcterms:issued>
        <dcterms:modified rdf:datatype="&xsd;date">2014-03-01+09:00</dcterms:modified>
        <skos:definition xml:lang="en">
    Aging is the process of storing beverages in casks for a specific period of
    time to remove harsh flavors and add distinct characteristics found in the
    cask&apos;s wood.
    </skos:definition>
        <skos:prefLabel xml:lang="en">Aging</skos:prefLabel>
        <status:term_status xml:lang="en">unstable</status:term_status>
        <skos:prefLabel xml:lang="ko">숙성</skos:prefLabel>
        <rdfs:isDefinedBy rdf:resource="http://rdfs.co/bevon/"/>
    </owl:Class>
    


    <!-- http://rdfs.co/bevon/AlcoholicBeverage -->

    <owl:Class rdf:about="&bevon;AlcoholicBeverage">
        <rdfs:subClassOf rdf:resource="&bevon;Beverage"/>
        <rdfs:subClassOf rdf:resource="&pto;Alcoholic_beverage"/>
        <owl:disjointWith rdf:resource="&bevon;NonAlcoholicBeverage"/>
        <dcterms:issued rdf:datatype="&xsd;date">2013-07-04+09:00</dcterms:issued>
        <dcterms:modified rdf:datatype="&xsd;date">2014-03-01+09:00</dcterms:modified>
        <skos:definition xml:lang="en">
     An alcoholic beverage is a drink and psychoactive drug containing
     ethyl alcohol which is commonly referred to as ethanol.
     </skos:definition>
        <skos:prefLabel xml:lang="en">Alcoholic Beverage</skos:prefLabel>
        <status:term_status xml:lang="en">testing</status:term_status>
        <skos:prefLabel xml:lang="ko">알코올 음료</skos:prefLabel>
        <rdfs:seeAlso rdf:resource="http://en.wikipedia.org/wiki/Alcoholic_beverage"/>
        <rdfs:isDefinedBy rdf:resource="http://rdfs.co/bevon/"/>
    </owl:Class>
    


    <!-- http://rdfs.co/bevon/Ale -->

    <owl:Class rdf:about="&bevon;Ale">
        <rdfs:subClassOf rdf:resource="&bevon;Beer"/>
        <rdfs:subClassOf rdf:resource="&pto;Ale"/>
        <dcterms:issued rdf:datatype="&xsd;date">2013-07-04+09:00</dcterms:issued>
        <dcterms:modified rdf:datatype="&xsd;date">2014-03-01+09:00</dcterms:modified>
        <skos:definition xml:lang="en">
    Ale is a type of beer brewed from malted barley using a warm-fermentation
    with a strain of brewers&apos; yeast.
    </skos:definition>
        <rdfs:comment xml:lang="en">
    The yeast will ferment the beer quickly, giving it a sweet, full bodied and
    fruity taste.
    </rdfs:comment>
        <skos:prefLabel xml:lang="en">Ale</skos:prefLabel>
        <status:term_status xml:lang="en">unstable</status:term_status>
        <skos:prefLabel xml:lang="ko">에일</skos:prefLabel>
        <rdfs:seeAlso rdf:resource="http://en.wikipedia.org/wiki/Ale"/>
        <rdfs:isDefinedBy rdf:resource="http://rdfs.co/bevon/"/>
    </owl:Class>
    


    <!-- http://rdfs.co/bevon/AmericanWhiskey -->

    <owl:Class rdf:about="&bevon;AmericanWhiskey">
        <rdfs:subClassOf rdf:resource="&bevon;Whisky"/>
        <rdfs:subClassOf rdf:resource="&pto;American_whiskey"/>
        <dcterms:issued rdf:datatype="&xsd;date">2013-07-04+09:00</dcterms:issued>
        <dcterms:modified rdf:datatype="&xsd;date">2014-03-01+09:00</dcterms:modified>
        <skos:definition xml:lang="en">
    American whiskey is a distilled beverage produced in the United States from
    a fermented mash of cereal grain.
    </skos:definition>
        <rdfs:comment xml:lang="en">
    The production and labeling of American whiskey are governed by Title 27 of
    the U.S. Code of Federal Regulations.
    </rdfs:comment>
        <skos:prefLabel xml:lang="en">American Whiskey</skos:prefLabel>
        <skos:altLabel xml:lang="en">American Whisky</skos:altLabel>
        <status:term_status xml:lang="en">unstable</status:term_status>
        <skos:prefLabel xml:lang="ko">아메리칸 위스키</skos:prefLabel>
        <rdfs:seeAlso rdf:resource="http://en.wikipedia.org/wiki/American_whiskey"/>
        <rdfs:isDefinedBy rdf:resource="http://rdfs.co/bevon/"/>
    </owl:Class>
    


    <!-- http://rdfs.co/bevon/AmericanWhisky -->

    <owl:Class rdf:about="&bevon;AmericanWhisky"/>
    


    <!-- http://rdfs.co/bevon/Beer -->

    <owl:Class rdf:about="&bevon;Beer">
        <rdfs:subClassOf rdf:resource="&bevon;FermentedBeverage"/>
        <rdfs:subClassOf rdf:resource="&pto;Beer"/>
        <owl:disjointWith rdf:resource="&bevon;NonAlcoholicBeer"/>
        <dcterms:issued rdf:datatype="&xsd;date">2013-07-04+09:00</dcterms:issued>
        <dcterms:modified rdf:datatype="&xsd;date">2014-03-01+09:00</dcterms:modified>
        <skos:definition xml:lang="en">
    Beer is an alcoholic beverage produced by the saccharification of starch and
    fermentation of the resulting sugar.
    </skos:definition>
        <rdfs:comment xml:lang="en">
    The starch and saccharification enzymes are often derived from malted cereal
    grains, most commonly malted barley and malted wheat.
    </rdfs:comment>
        <skos:prefLabel xml:lang="en">Beer</skos:prefLabel>
        <status:term_status xml:lang="en">testing</status:term_status>
        <skos:prefLabel xml:lang="ko">맥주</skos:prefLabel>
        <rdfs:seeAlso rdf:resource="http://en.wikipedia.org/wiki/Beer"/>
        <rdfs:isDefinedBy rdf:resource="http://rdfs.co/bevon/"/>
    </owl:Class>
    


    <!-- http://rdfs.co/bevon/BeerBottle -->

    <owl:Class rdf:about="&bevon;BeerBottle">
        <rdfs:subClassOf rdf:resource="&bevon;GlassBottle"/>
        <dcterms:issued rdf:datatype="&xsd;date">2013-07-04+09:00</dcterms:issued>
        <dcterms:modified rdf:datatype="&xsd;date">2014-03-01+09:00</dcterms:modified>
        <skos:definition xml:lang="en">
    A beer bottle is a bottle made to contain beer, usually made of glass and
    come in various sizes, shapes and colors.
    </skos:definition>
        <rdfs:comment xml:lang="en">
    Dark amber or brown glass greatly reduces UV light from spoiling the beer.
    However, lighter colored bottles are often used for marketing reasons.
    </rdfs:comment>
        <skos:prefLabel xml:lang="en">Beer Bottle</skos:prefLabel>
        <status:term_status xml:lang="en">unstable</status:term_status>
        <skos:prefLabel xml:lang="ko">맥주병</skos:prefLabel>
        <rdfs:seeAlso rdf:resource="http://en.wikipedia.org/wiki/Beer_bottle"/>
        <rdfs:isDefinedBy rdf:resource="http://rdfs.co/bevon/"/>
    </owl:Class>
    


    <!-- http://rdfs.co/bevon/BeerCocktail -->

    <owl:Class rdf:about="&bevon;BeerCocktail">
        <rdfs:subClassOf rdf:resource="&bevon;Cocktail"/>
        <rdfs:subClassOf rdf:resource="&pto;Beer_cocktail"/>
        <dcterms:issued rdf:datatype="&xsd;date">2013-07-04+09:00</dcterms:issued>
        <dcterms:modified rdf:datatype="&xsd;date">2014-03-01+09:00</dcterms:modified>
        <skos:definition xml:lang="en">
    A beer cocktail is a cocktail that is made by mixing beer with a distilled
    beverage. In this type of cocktail, the primary ingredient is beer.
    </skos:definition>
        <skos:prefLabel xml:lang="en">Beer Cocktail</skos:prefLabel>
        <status:term_status xml:lang="en">unstable</status:term_status>
        <skos:prefLabel xml:lang="ko">맥주 칵테일</skos:prefLabel>
        <rdfs:seeAlso rdf:resource="http://en.wikipedia.org/wiki/Beer_cocktail"/>
        <rdfs:isDefinedBy rdf:resource="http://rdfs.co/bevon/"/>
    </owl:Class>
    


    <!-- http://rdfs.co/bevon/BeerKeg -->

    <owl:Class rdf:about="&bevon;BeerKeg">
        <rdfs:subClassOf rdf:resource="&bevon;Keg"/>
        <dcterms:issued rdf:datatype="&xsd;date">2013-07-04+09:00</dcterms:issued>
        <dcterms:modified rdf:datatype="&xsd;date">2014-03-01+09:00</dcterms:modified>
        <skos:definition xml:lang="en">
    Beer kegs are made of stainless steel, or less commonly, of aluminium.
    </skos:definition>
        <skos:prefLabel xml:lang="en">Beer Keg</skos:prefLabel>
        <status:term_status xml:lang="en">unstable</status:term_status>
        <skos:prefLabel xml:lang="ko">맥주 케그</skos:prefLabel>
        <rdfs:isDefinedBy rdf:resource="http://rdfs.co/bevon/"/>
    </owl:Class>
    


    <!-- http://rdfs.co/bevon/Beverage -->

    <owl:Class rdf:about="&bevon;Beverage">
        <rdfs:subClassOf rdf:resource="&food;Food"/>
        <rdfs:subClassOf rdf:resource="&pto;Drink"/>
        <rdfs:subClassOf rdf:resource="&fowl;PotableLiquid"/>
        <dcterms:issued rdf:datatype="&xsd;date">2013-07-04+09:00</dcterms:issued>
        <dcterms:modified rdf:datatype="&xsd;date">2014-03-01+09:00</dcterms:modified>
        <skos:definition xml:lang="en">
    A beverage, or drink, is a kind of liquid which is specifically prepared
    for human consumption.
    </skos:definition>
        <skos:prefLabel xml:lang="en">Beverage</skos:prefLabel>
        <skos:altLabel xml:lang="en">Drink</skos:altLabel>
        <status:term_status xml:lang="en">testing</status:term_status>
        <skos:prefLabel xml:lang="ko">음료</skos:prefLabel>
        <rdfs:seeAlso rdf:resource="http://en.wikipedia.org/wiki/Beverage"/>
        <rdfs:isDefinedBy rdf:resource="http://rdfs.co/bevon/"/>
    </owl:Class>
    


    <!-- http://rdfs.co/bevon/BeverageCan -->

    <owl:Class rdf:about="&bevon;BeverageCan">
        <rdfs:subClassOf rdf:resource="&bevon;Container"/>
        <dcterms:issued rdf:datatype="&xsd;date">2013-07-04+09:00</dcterms:issued>
        <dcterms:modified rdf:datatype="&xsd;date">2014-03-01+09:00</dcterms:modified>
        <skos:definition xml:lang="en">
    A beverage can is a metal container designed to hold a fixed portion of
    liquid such as a carbonated soft drinks, alcoholic beverages, fruit juices,
    teas, tisanes, energy drinks, etc.
    </skos:definition>
        <rdfs:comment xml:lang="en">
    Beverage cans are made of aluminium (75% of worldwide production) or
    tin-plated steel (25% worldwide production).
    </rdfs:comment>
        <skos:prefLabel xml:lang="en">Beverage Can</skos:prefLabel>
        <status:term_status xml:lang="en">unstable</status:term_status>
        <skos:prefLabel xml:lang="ko">음료 캔</skos:prefLabel>
        <rdfs:seeAlso rdf:resource="http://en.wikipedia.org/wiki/Beverage_can"/>
        <rdfs:isDefinedBy rdf:resource="http://rdfs.co/bevon/"/>
    </owl:Class>
    


    <!-- http://rdfs.co/bevon/BourbonWhiskey -->

    <owl:Class rdf:about="&bevon;BourbonWhiskey">
        <rdfs:subClassOf rdf:resource="&bevon;AmericanWhisky"/>
        <rdfs:subClassOf rdf:resource="&pto;Bourbon_whiskey"/>
        <dcterms:issued rdf:datatype="&xsd;date">2013-07-04+09:00</dcterms:issued>
        <dcterms:modified rdf:datatype="&xsd;date">2014-03-01+09:00</dcterms:modified>
        <skos:definition xml:lang="en">
    Bourbon whiskey is a type of American whiskey – a barrel-aged distilled
    spirit made primarily from corn.
    </skos:definition>
        <rdfs:comment xml:lang="en">
    The name of the spirit derives from its historical association with an area
    known as Old Bourbon, around what is now Bourbon County, Kentucky (which,
    in turn, was named after the French House of Bourbon royal family). It has
    been produced since the 18th century. While it may be made anywhere in the
    United States, it is strongly associated with the American South in
    general, and Kentucky in particular.
    </rdfs:comment>
        <skos:prefLabel xml:lang="en">Bourbon Whiskey</skos:prefLabel>
        <skos:altLabel xml:lang="en">Bourbon Whisky</skos:altLabel>
        <status:term_status xml:lang="en">unstable</status:term_status>
        <skos:prefLabel xml:lang="ko">버번 위스키</skos:prefLabel>
        <rdfs:seeAlso rdf:resource="http://en.wikipedia.org/wiki/Bourbon_whiskey"/>
        <rdfs:isDefinedBy rdf:resource="http://rdfs.co/bevon/"/>
    </owl:Class>
    


    <!-- http://rdfs.co/bevon/Brandy -->

    <owl:Class rdf:about="&bevon;Brandy">
        <rdfs:subClassOf rdf:resource="&bevon;DistilledBeverage"/>
        <rdfs:subClassOf rdf:resource="&pto;Brandy"/>
        <dcterms:issued rdf:datatype="&xsd;date">2013-07-04+09:00</dcterms:issued>
        <dcterms:modified rdf:datatype="&xsd;date">2014-03-01+09:00</dcterms:modified>
        <skos:definition xml:lang="en">
    Brandy (from brandywine, derived from Dutch brandewijn—&quot;burnt wine&quot;) is a
    spirit produced by distilling wine.
    </skos:definition>
        <rdfs:comment xml:lang="en">
    Brandy generally contains 35–60% alcohol by volume (70–120 US proof) and is
    typically taken as an after-dinner drink. Some brandies are aged in wooden
    casks, some are colored with caramel coloring to imitate the effect of
    aging, and some brandies are produced using a combination of both aging and
    coloring.
    </rdfs:comment>
        <skos:prefLabel xml:lang="en">Brandy</skos:prefLabel>
        <status:term_status xml:lang="en">testing</status:term_status>
        <skos:prefLabel xml:lang="ko">브랜디</skos:prefLabel>
        <rdfs:seeAlso rdf:resource="http://en.wikipedia.org/wiki/Brandy"/>
        <rdfs:isDefinedBy rdf:resource="http://rdfs.co/bevon/"/>
    </owl:Class>
    


    <!-- http://rdfs.co/bevon/Brewery -->

    <owl:Class rdf:about="&bevon;Brewery">
        <dcterms:issued rdf:datatype="&xsd;date">2013-07-04+09:00</dcterms:issued>
        <dcterms:modified rdf:datatype="&xsd;date">2014-03-01+09:00</dcterms:modified>
        <skos:definition xml:lang="en">
    A brewery is a dedicated building for the making of beer, though beer can
    be made at home, and has been for much of beer&apos;s history.
    </skos:definition>
        <rdfs:comment xml:lang="en">
    A company that makes beer is called either a brewery or a brewing company.
    </rdfs:comment>
        <skos:prefLabel xml:lang="en">Brewery</skos:prefLabel>
        <status:term_status xml:lang="en">unstable</status:term_status>
        <skos:prefLabel xml:lang="ko">양조장</skos:prefLabel>
        <rdfs:seeAlso rdf:resource="http://en.wikipedia.org/wiki/Brewery"/>
        <rdfs:isDefinedBy rdf:resource="http://rdfs.co/bevon/"/>
    </owl:Class>
    


    <!-- http://rdfs.co/bevon/CanadianWhisky -->

    <owl:Class rdf:about="&bevon;CanadianWhisky">
        <rdfs:subClassOf rdf:resource="&bevon;Whisky"/>
        <rdfs:subClassOf rdf:resource="&pto;Canadian_whisky"/>
        <dcterms:issued rdf:datatype="&xsd;date">2013-07-04+09:00</dcterms:issued>
        <dcterms:modified rdf:datatype="&xsd;date">2014-03-01+09:00</dcterms:modified>
        <skos:definition xml:lang="en">
    Canadian whisky is a type of whisky produced in Canada.
    </skos:definition>
        <rdfs:comment xml:lang="en">
    Most Canadian whiskies are blended multi-grain liquors containing a large
    percentage of corn spirits, and are typically lighter and smoother than
    other whisky styles.
    </rdfs:comment>
        <skos:altLabel xml:lang="en">Canadian Whiskey</skos:altLabel>
        <skos:prefLabel xml:lang="en">Canadian Whisky</skos:prefLabel>
        <status:term_status xml:lang="en">unstable</status:term_status>
        <skos:prefLabel xml:lang="ko">캐내디언 위스키</skos:prefLabel>
        <rdfs:seeAlso rdf:resource="http://en.wikipedia.org/wiki/Canadian_whisky"/>
        <rdfs:isDefinedBy rdf:resource="http://rdfs.co/bevon/"/>
    </owl:Class>
    


    <!-- http://rdfs.co/bevon/CarbonatedWater -->

    <owl:Class rdf:about="&bevon;CarbonatedWater">
        <rdfs:subClassOf rdf:resource="&bevon;Water"/>
        <rdfs:subClassOf rdf:resource="&pto;Carbonated_water"/>
        <dcterms:issued rdf:datatype="&xsd;date">2013-07-04+09:00</dcterms:issued>
        <dcterms:modified rdf:datatype="&xsd;date">2014-03-01+09:00</dcterms:modified>
        <skos:definition xml:lang="en">
    Carbonated water is water into which carbon dioxide gas under pressure has
    been dissolved.
    </skos:definition>
        <skos:prefLabel xml:lang="en">Carbonated Water</skos:prefLabel>
        <skos:altLabel xml:lang="en">Club Soda</skos:altLabel>
        <skos:altLabel xml:lang="en">Fizzy Water</skos:altLabel>
        <skos:altLabel xml:lang="en">Seltzer Water</skos:altLabel>
        <skos:altLabel xml:lang="en">Soda Water</skos:altLabel>
        <skos:altLabel xml:lang="en">Sparkling Water</skos:altLabel>
        <status:term_status xml:lang="en">unstable</status:term_status>
        <skos:altLabel xml:lang="ko">소다수</skos:altLabel>
        <skos:altLabel xml:lang="ko">클럽소다</skos:altLabel>
        <skos:prefLabel xml:lang="ko">탄산수</skos:prefLabel>
        <rdfs:seeAlso rdf:resource="http://en.wikipedia.org/wiki/Carbonated_water"/>
        <rdfs:isDefinedBy rdf:resource="http://rdfs.co/bevon/"/>
    </owl:Class>
    


    <!-- http://rdfs.co/bevon/Cocktail -->

    <owl:Class rdf:about="&bevon;Cocktail">
        <rdfs:subClassOf rdf:resource="&bevon;AlcoholicBeverage"/>
        <rdfs:subClassOf rdf:resource="&bevon;MixedDrink"/>
        <rdfs:subClassOf rdf:resource="&pto;Cocktail"/>
        <owl:disjointWith rdf:resource="&bevon;Mocktail"/>
        <dcterms:issued rdf:datatype="&xsd;date">2013-07-04+09:00</dcterms:issued>
        <dcterms:modified rdf:datatype="&xsd;date">2014-03-01+09:00</dcterms:modified>
        <skos:definition xml:lang="en">
    A cocktail is a mixed drink that contains alcohol, including mixers, mixed
    shots, etc.
    </skos:definition>
        <rdfs:comment xml:lang="en">
    Cocktails were originally a mixture of spirits, sugar, water, and bitters.
    It is now often used for almost any mixed drink that contains alcohol,
    including mixers, mixed shots, etc. A cocktail today usually contains one
    or more kinds of spirit and one or more mixers, such as soda or fruit juice.
    Additional ingredients may be sugar, honey, milk, cream, and various herbs.
    </rdfs:comment>
        <skos:prefLabel xml:lang="en">Cocktail</skos:prefLabel>
        <status:term_status xml:lang="en">unstable</status:term_status>
        <skos:prefLabel xml:lang="ko">칵테일</skos:prefLabel>
        <rdfs:seeAlso rdf:resource="http://en.wikipedia.org/wiki/Cocktail"/>
        <rdfs:isDefinedBy rdf:resource="http://rdfs.co/bevon/"/>
    </owl:Class>
    


    <!-- http://rdfs.co/bevon/Cognac -->

    <owl:Class rdf:about="&bevon;Cognac">
        <rdfs:subClassOf rdf:resource="&bevon;Brandy"/>
        <rdfs:subClassOf rdf:resource="&pto;Cognac"/>
        <dcterms:issued rdf:datatype="&xsd;date">2013-07-04+09:00</dcterms:issued>
        <dcterms:modified rdf:datatype="&xsd;date">2014-03-01+09:00</dcterms:modified>
        <skos:definition xml:lang="en">
    Cognac, named after the town of Cognac in France, is a variety of brandy.
    </skos:definition>
        <rdfs:comment xml:lang="en">
    It is produced in the wine-growing region surrounding the town from which
    it takes its name, in the French Departements of Charente and
    Charente-Maritime.
    </rdfs:comment>
        <skos:prefLabel xml:lang="en">Cognac</skos:prefLabel>
        <status:term_status xml:lang="en">testing</status:term_status>
        <skos:prefLabel xml:lang="ko">코냑</skos:prefLabel>
        <rdfs:seeAlso rdf:resource="http://en.wikipedia.org/wiki/Cognac"/>
        <rdfs:isDefinedBy rdf:resource="http://rdfs.co/bevon/"/>
    </owl:Class>
    


    <!-- http://rdfs.co/bevon/Container -->

    <owl:Class rdf:about="&bevon;Container">
        <rdfs:subClassOf rdf:resource="&yago;Containers"/>
        <dcterms:issued rdf:datatype="&xsd;date">2013-07-04+09:00</dcterms:issued>
        <dcterms:modified rdf:datatype="&xsd;date">2014-03-01+09:00</dcterms:modified>
        <skos:definition xml:lang="en">
    A container is an item used to contain, store, and transport a beverage.
    </skos:definition>
        <skos:prefLabel xml:lang="en">Container</skos:prefLabel>
        <status:term_status xml:lang="en">unstable</status:term_status>
        <skos:prefLabel xml:lang="ko">용기</skos:prefLabel>
        <rdfs:seeAlso rdf:resource="http://en.wikipedia.org/wiki/Container"/>
        <rdfs:isDefinedBy rdf:resource="http://rdfs.co/bevon/"/>
    </owl:Class>
    


    <!-- http://rdfs.co/bevon/DilutedSoju -->

    <owl:Class rdf:about="&bevon;DilutedSoju">
        <rdfs:subClassOf rdf:resource="&bevon;Soju"/>
        <owl:disjointWith rdf:resource="&bevon;DistilledSoju"/>
        <dcterms:issued rdf:datatype="&xsd;date">2013-07-04+09:00</dcterms:issued>
        <dcterms:modified rdf:datatype="&xsd;date">2014-03-01+09:00</dcterms:modified>
        <skos:definition xml:lang="en">
    Diluted Soju is made by mixing pure ethanol distilled from various grains,
    such as potatoes, wheat, barley, sweet potatoes, or tapioca, with water and
    flavoring.
    </skos:definition>
        <skos:prefLabel xml:lang="en">Diluted Soju</skos:prefLabel>
        <status:term_status xml:lang="en">unstable</status:term_status>
        <skos:prefLabel xml:lang="ko">희석식 소주</skos:prefLabel>
        <rdfs:isDefinedBy rdf:resource="http://rdfs.co/bevon/"/>
    </owl:Class>
    


    <!-- http://rdfs.co/bevon/DistilledBeverage -->

    <owl:Class rdf:about="&bevon;DistilledBeverage">
        <rdfs:subClassOf rdf:resource="&bevon;AlcoholicBeverage"/>
        <rdfs:subClassOf rdf:resource="&pto;Distilled_beverage"/>
        <dcterms:issued rdf:datatype="&xsd;date">2013-07-04+09:00</dcterms:issued>
        <dcterms:modified rdf:datatype="&xsd;date">2014-03-01+09:00</dcterms:modified>
        <skos:definition xml:lang="en">
     A distilled beverage, spirit, or liquor is an alcoholic beverage
     containing ethanol that is produced by distilling (i.e., concentrating
     by distillation) ethanol produced by means of fermenting grain, fruit,
     or vegetables.
     </skos:definition>
        <rdfs:comment xml:lang="en">
     This excludes undistilled fermented beverages such as beer, wine, and
     cider.
     </rdfs:comment>
        <skos:prefLabel xml:lang="en">Distilled Beverage</skos:prefLabel>
        <skos:altLabel xml:lang="en">Liquor</skos:altLabel>
        <skos:altLabel xml:lang="en">Spirit</skos:altLabel>
        <status:term_status xml:lang="en">testing</status:term_status>
        <skos:prefLabel xml:lang="ko">증류주</skos:prefLabel>
        <rdfs:seeAlso rdf:resource="http://en.wikipedia.org/wiki/Distilled_beverage"/>
        <rdfs:isDefinedBy rdf:resource="http://rdfs.co/bevon/"/>
    </owl:Class>
    


    <!-- http://rdfs.co/bevon/DistilledSoju -->

    <owl:Class rdf:about="&bevon;DistilledSoju">
        <rdfs:subClassOf rdf:resource="&bevon;Soju"/>
        <dcterms:issued rdf:datatype="&xsd;date">2013-07-04+09:00</dcterms:issued>
        <dcterms:modified rdf:datatype="&xsd;date">2014-03-01+09:00</dcterms:modified>
        <skos:definition xml:lang="en">
    Distilled Soju is manufactured traditionally by distillation from grains,
    mainly rice.
    </skos:definition>
        <skos:prefLabel xml:lang="en">Distilled Soju</skos:prefLabel>
        <status:term_status xml:lang="en">unstable</status:term_status>
        <skos:prefLabel xml:lang="ko">증류식 소주</skos:prefLabel>
        <rdfs:isDefinedBy rdf:resource="http://rdfs.co/bevon/"/>
    </owl:Class>
    


    <!-- http://rdfs.co/bevon/Distillery -->

    <owl:Class rdf:about="&bevon;Distillery">
        <dcterms:issued rdf:datatype="&xsd;date">2013-07-04+09:00</dcterms:issued>
        <dcterms:modified rdf:datatype="&xsd;date">2014-03-01+09:00</dcterms:modified>
        <skos:definition xml:lang="en">
    A distillery is a premise where distillation takes place, especially
    distillation of alcohol.
    </skos:definition>
        <skos:prefLabel xml:lang="en">Distillery</skos:prefLabel>
        <status:term_status xml:lang="en">unstable</status:term_status>
        <skos:prefLabel xml:lang="ko">증류소</skos:prefLabel>
        <rdfs:seeAlso rdf:resource="http://en.wikipedia.org/wiki/Distillation"/>
        <rdfs:isDefinedBy rdf:resource="http://rdfs.co/bevon/"/>
    </owl:Class>
    


    <!-- http://rdfs.co/bevon/DryStout -->

    <owl:Class rdf:about="&bevon;DryStout">
        <rdfs:subClassOf rdf:resource="&bevon;Stout"/>
        <dcterms:issued rdf:datatype="&xsd;date">2013-07-04+09:00</dcterms:issued>
        <dcterms:modified rdf:datatype="&xsd;date">2014-03-01+09:00</dcterms:modified>
        <skos:definition xml:lang="en">
    Irish stout or dry stout is very dark or rich in color and it often has a
    &quot;roasted&quot; or coffee-like taste.
    </skos:definition>
        <skos:prefLabel xml:lang="en">Dry Stout</skos:prefLabel>
        <skos:altLabel xml:lang="en">Irish Stout</skos:altLabel>
        <status:term_status xml:lang="en">unstable</status:term_status>
        <skos:prefLabel xml:lang="ko">드라이 스타우트</skos:prefLabel>
        <rdfs:isDefinedBy rdf:resource="http://rdfs.co/bevon/"/>
    </owl:Class>
    


    <!-- http://rdfs.co/bevon/Dunkel -->

    <owl:Class rdf:about="&bevon;Dunkel">
        <rdfs:subClassOf rdf:resource="&bevon;Lager"/>
        <rdfs:subClassOf rdf:resource="&pto;Dunkel"/>
        <dcterms:issued rdf:datatype="&xsd;date">2013-07-04+09:00</dcterms:issued>
        <dcterms:modified rdf:datatype="&xsd;date">2014-03-01+09:00</dcterms:modified>
        <rdfs:comment xml:lang="en">
    Dunkel is the German word meaning dark, and dunkel beers typically range in
    color from amber to dark reddish brown. They are characterized by their
    smooth malty flavor.
    </rdfs:comment>
        <skos:definition xml:lang="en">
    Dunkel, or Dunkles, is a word used for several types of dark German lager.
    </skos:definition>
        <skos:prefLabel xml:lang="en">Dunkel</skos:prefLabel>
        <skos:altLabel xml:lang="en">Dunkles</skos:altLabel>
        <status:term_status xml:lang="en">unstable</status:term_status>
        <skos:prefLabel xml:lang="ko">둔켈</skos:prefLabel>
        <rdfs:isDefinedBy rdf:resource="http://rdfs.co/bevon/"/>
        <rdfs:seeAlso rdf:resource="https://en.wikipedia.org/wiki/Dunkel"/>
    </owl:Class>
    


    <!-- http://rdfs.co/bevon/FermentationBase -->

    <owl:Class rdf:about="&bevon;FermentationBase">
        <dcterms:issued rdf:datatype="&xsd;date">2013-07-04+09:00</dcterms:issued>
        <dcterms:modified rdf:datatype="&xsd;date">2014-03-01+09:00</dcterms:modified>
        <skos:definition xml:lang="en">
    A fruit or grain which provides the sugar for fermentation from which a
    alcoholic beverage is made.
    </skos:definition>
        <skos:prefLabel xml:lang="en">Fermentation Base</skos:prefLabel>
        <status:term_status xml:lang="en">unstable</status:term_status>
        <skos:prefLabel xml:lang="ko">발효 주재료</skos:prefLabel>
        <rdfs:isDefinedBy rdf:resource="http://rdfs.co/bevon/"/>
    </owl:Class>
    


    <!-- http://rdfs.co/bevon/FermentedBeverage -->

    <owl:Class rdf:about="&bevon;FermentedBeverage">
        <rdfs:subClassOf rdf:resource="&bevon;AlcoholicBeverage"/>
        <dcterms:issued rdf:datatype="&xsd;date">2013-07-04+09:00</dcterms:issued>
        <dcterms:modified rdf:datatype="&xsd;date">2014-03-01+09:00</dcterms:modified>
        <skos:definition xml:lang="en">
    A fermented beverage is a drink produced by fermenting grain, fruit, or
    vegetables.
    </skos:definition>
        <skos:prefLabel xml:lang="en">Fermented Beverage</skos:prefLabel>
        <status:term_status xml:lang="en">testing</status:term_status>
        <skos:altLabel xml:lang="ko">발효주</skos:altLabel>
        <skos:prefLabel xml:lang="ko">양조주</skos:prefLabel>
        <rdfs:isDefinedBy rdf:resource="http://rdfs.co/bevon/"/>
    </owl:Class>
    


    <!-- http://rdfs.co/bevon/FruitWine -->

    <owl:Class rdf:about="&bevon;FruitWine">
        <rdfs:subClassOf rdf:resource="&bevon;Wine"/>
        <rdfs:subClassOf rdf:resource="&pto;Fruit_wine"/>
        <dcterms:issued rdf:datatype="&xsd;date">2014-03-07+09:00</dcterms:issued>
        <dcterms:modified rdf:datatype="&xsd;date">2014-03-07+09:00</dcterms:modified>
        <skos:definition xml:lang="en">
    Fruit wines are fermented alcoholic beverages made from a variety of base
    ingredients (other than grapes); they may also have additional flavors
    taken from fruits, flowers, and herbs.
    </skos:definition>
        <rdfs:comment xml:lang="en">
    This definition is sometimes broadened to include any fermented alcoholic
    beverage except beer. For historical reasons, mead, cider, and perry are
    also excluded from the definition of fruit wine.
    </rdfs:comment>
        <skos:prefLabel xml:lang="en">Fruit Wine</skos:prefLabel>
        <status:term_status xml:lang="en">testing</status:term_status>
        <skos:prefLabel xml:lang="fr">Vin de Sureau</skos:prefLabel>
        <skos:prefLabel xml:lang="ko">과실주</skos:prefLabel>
        <rdfs:seeAlso rdf:resource="http://en.wikipedia.org/wiki/Fruit_wine"/>
        <rdfs:isDefinedBy rdf:resource="http://rdfs.co/bevon/"/>
    </owl:Class>
    


    <!-- http://rdfs.co/bevon/Gin -->

    <owl:Class rdf:about="&bevon;Gin">
        <rdfs:subClassOf rdf:resource="&bevon;DistilledBeverage"/>
        <rdfs:subClassOf rdf:resource="&pto;Gin"/>
        <dcterms:issued rdf:datatype="&xsd;date">2013-07-04+09:00</dcterms:issued>
        <dcterms:modified rdf:datatype="&xsd;date">2014-03-01+09:00</dcterms:modified>
        <skos:definition xml:lang="en">
    Gin is a spirit which derives its predominant flavor from juniper berries
    (Juniperus communis).
    </skos:definition>
        <skos:prefLabel xml:lang="en">Gin</skos:prefLabel>
        <status:term_status xml:lang="en">testing</status:term_status>
        <skos:prefLabel xml:lang="ko">진</skos:prefLabel>
        <rdfs:seeAlso rdf:resource="http://en.wikipedia.org/wiki/Gin"/>
        <rdfs:isDefinedBy rdf:resource="http://rdfs.co/bevon/"/>
    </owl:Class>
    


    <!-- http://rdfs.co/bevon/GlassBottle -->

    <owl:Class rdf:about="&bevon;GlassBottle">
        <rdfs:subClassOf rdf:resource="&bevon;Container"/>
        <dcterms:issued rdf:datatype="&xsd;date">2013-07-04+09:00</dcterms:issued>
        <dcterms:modified rdf:datatype="&xsd;date">2014-03-01+09:00</dcterms:modified>
        <skos:definition xml:lang="en">
    A glass bottle is a bottle created from glass.
    </skos:definition>
        <rdfs:comment xml:lang="en">
    Glass bottles can vary in size considerably, but are most commonly found in
    sizes ranging between about 10ml and 5 litres.
    </rdfs:comment>
        <skos:prefLabel xml:lang="en">Glass Bottle</skos:prefLabel>
        <status:term_status xml:lang="en">unstable</status:term_status>
        <skos:prefLabel xml:lang="ko">유리병</skos:prefLabel>
        <rdfs:seeAlso rdf:resource="http://en.wikipedia.org/wiki/Glass_bottle"/>
        <rdfs:isDefinedBy rdf:resource="http://rdfs.co/bevon/"/>
    </owl:Class>
    


    <!-- http://rdfs.co/bevon/Highball -->

    <owl:Class rdf:about="&bevon;Highball">
        <rdfs:subClassOf rdf:resource="&bevon;Cocktail"/>
        <rdfs:subClassOf rdf:resource="&pto;Highball"/>
        <dcterms:issued rdf:datatype="&xsd;date">2013-07-04+09:00</dcterms:issued>
        <dcterms:modified rdf:datatype="&xsd;date">2014-03-01+09:00</dcterms:modified>
        <skos:definition xml:lang="en">
    Highball is the name for a family of mixed drinks that are composed of an
    alcoholic base spirit and a larger proportion of a non-alcoholic mixer.
    </skos:definition>
        <skos:prefLabel xml:lang="en">Highball</skos:prefLabel>
        <status:term_status xml:lang="en">unstable</status:term_status>
        <skos:prefLabel xml:lang="ko">하이볼</skos:prefLabel>
        <rdfs:seeAlso rdf:resource="http://en.wikipedia.org/wiki/Highball"/>
        <rdfs:isDefinedBy rdf:resource="http://rdfs.co/bevon/"/>
    </owl:Class>
    


    <!-- http://rdfs.co/bevon/IrishRedAle -->

    <owl:Class rdf:about="&bevon;IrishRedAle">
        <rdfs:subClassOf rdf:resource="&bevon;PaleAle"/>
        <dcterms:issued rdf:datatype="&xsd;date">2013-07-04+09:00</dcterms:issued>
        <dcterms:modified rdf:datatype="&xsd;date">2014-03-01+09:00</dcterms:modified>
        <skos:definition xml:lang="en">
    Irish red ale, red ale, or Irish ale is a name used by brewers in Ireland.
    </skos:definition>
        <skos:prefLabel xml:lang="en">Irish Red Ale</skos:prefLabel>
        <status:term_status xml:lang="en">unstable</status:term_status>
        <skos:prefLabel xml:lang="ko">아이리쉬 레드 에일</skos:prefLabel>
        <rdfs:seeAlso rdf:resource="http://en.wikipedia.org/wiki/Irish_red_ale"/>
        <rdfs:isDefinedBy rdf:resource="http://rdfs.co/bevon/"/>
    </owl:Class>
    


    <!-- http://rdfs.co/bevon/IrishWhiskey -->

    <owl:Class rdf:about="&bevon;IrishWhiskey">
        <rdfs:subClassOf rdf:resource="&bevon;Whisky"/>
        <rdfs:subClassOf rdf:resource="&pto;Irish_whiskey"/>
        <dcterms:issued rdf:datatype="&xsd;date">2013-07-04+09:00</dcterms:issued>
        <dcterms:modified rdf:datatype="&xsd;date">2014-03-01+09:00</dcterms:modified>
        <skos:definition xml:lang="en">
    Irish whiskey is whisky made in Ireland.
    </skos:definition>
        <rdfs:comment xml:lang="en">
    Key regulations defining Irish whiskey and its production are established
    by the Irish Whiskey Act of 1980.
    </rdfs:comment>
        <skos:prefLabel xml:lang="en">Irish Whiskey</skos:prefLabel>
        <skos:altLabel xml:lang="en">Irish Whisky</skos:altLabel>
        <status:term_status xml:lang="en">unstable</status:term_status>
        <skos:prefLabel xml:lang="ga">Fuisce</skos:prefLabel>
        <skos:prefLabel xml:lang="ko">아이리쉬 위스키</skos:prefLabel>
        <rdfs:seeAlso rdf:resource="http://en.wikipedia.org/wiki/Irish_whiskey"/>
        <rdfs:isDefinedBy rdf:resource="http://rdfs.co/bevon/"/>
    </owl:Class>
    


    <!-- http://rdfs.co/bevon/JapaneseWhisky -->

    <owl:Class rdf:about="&bevon;JapaneseWhisky">
        <rdfs:subClassOf rdf:resource="&bevon;Whisky"/>
        <rdfs:subClassOf rdf:resource="&pto;Japanese_whisky"/>
        <dcterms:issued rdf:datatype="&xsd;date">2013-07-04+09:00</dcterms:issued>
        <dcterms:modified rdf:datatype="&xsd;date">2014-03-01+09:00</dcterms:modified>
        <skos:definition xml:lang="en">
    Japanese whisky is whisky made in Japan.
    </skos:definition>
        <rdfs:commercial xml:lang="en">
    Whisky production in Japan began around 1870, but the first commercial
    production was in 1924 upon the opening of the country&apos;s first distillery,
    Yamazaki. Broadly speaking the style of Japanese whisky is more similar to
    that of Scotch whisky than Irish, American, or Canadian styles of whisky,
    and thus the spelling typically follows the Scottish convention (omitting
    the letter &quot;e&quot;).
    </rdfs:commercial>
        <skos:altLabel xml:lang="en">Japanese Whiskey</skos:altLabel>
        <skos:prefLabel xml:lang="en">Japanese Whisky</skos:prefLabel>
        <status:term_status xml:lang="en">unstable</status:term_status>
        <skos:prefLabel xml:lang="ko">재패니즈 위스키</skos:prefLabel>
        <rdfs:seeAlso rdf:resource="http://en.wikipedia.org/wiki/Japanese_whisky"/>
        <rdfs:isDefinedBy rdf:resource="http://rdfs.co/bevon/"/>
    </owl:Class>
    


    <!-- http://rdfs.co/bevon/Keg -->

    <owl:Class rdf:about="&bevon;Keg">
        <rdfs:subClassOf rdf:resource="&bevon;Container"/>
        <dcterms:issued rdf:datatype="&xsd;date">2013-07-04+09:00</dcterms:issued>
        <dcterms:modified rdf:datatype="&xsd;date">2014-03-01+09:00</dcterms:modified>
        <skos:definition xml:lang="en">
    A keg is a small barrel.
    </skos:definition>
        <skos:prefLabel xml:lang="en">Keg</skos:prefLabel>
        <status:term_status xml:lang="en">unstable</status:term_status>
        <skos:prefLabel xml:lang="ko">케그</skos:prefLabel>
        <rdfs:seeAlso rdf:resource="http://en.wikipedia.org/wiki/Keg"/>
        <rdfs:isDefinedBy rdf:resource="http://rdfs.co/bevon/"/>
    </owl:Class>
    


    <!-- http://rdfs.co/bevon/Lager -->

    <owl:Class rdf:about="&bevon;Lager">
        <rdfs:subClassOf rdf:resource="&bevon;Beer"/>
        <rdfs:subClassOf rdf:resource="&pto;Lager"/>
        <dcterms:issued rdf:datatype="&xsd;date">2013-07-04+09:00</dcterms:issued>
        <dcterms:modified rdf:datatype="&xsd;date">2014-03-01+09:00</dcterms:modified>
        <skos:definition xml:lang="en">
    Lager is a type of beer that is fermented and conditioned at low
    temperatures.
    </skos:definition>
        <skos:prefLabel xml:lang="en">Lager</skos:prefLabel>
        <status:term_status xml:lang="en">unstable</status:term_status>
        <skos:prefLabel xml:lang="ko">라거</skos:prefLabel>
        <rdfs:seeAlso rdf:resource="http://en.wikipedia.org/wiki/Lager"/>
        <rdfs:isDefinedBy rdf:resource="http://rdfs.co/bevon/"/>
    </owl:Class>
    


    <!-- http://rdfs.co/bevon/Liqueur -->

    <owl:Class rdf:about="&bevon;Liqueur">
        <rdfs:subClassOf rdf:resource="&bevon;DistilledBeverage"/>
        <rdfs:subClassOf rdf:resource="&pto;Liqueur"/>
        <dcterms:issued rdf:datatype="&xsd;date">2013-07-04+09:00</dcterms:issued>
        <dcterms:modified rdf:datatype="&xsd;date">2014-03-01+09:00</dcterms:modified>
        <skos:definition xml:lang="en">
    A liqueur is an alcoholic beverage made from a distilled spirit that has
    been flavored with fruit, cream, herbs, spices, flowers or nuts and bottled
    with added sugar or other sweetener (such as high-fructose corn syrup).
    </skos:definition>
        <rdfs:comment xml:lang="en">
    Liqueurs are typically quite sweet; they are usually not aged for long
    after the ingredients are mixed, but may have resting periods during their
    production to allow flavors to marry.
    </rdfs:comment>
        <skos:altLabel xml:lang="en">Cordials</skos:altLabel>
        <skos:prefLabel xml:lang="en">Liqueur</skos:prefLabel>
        <skos:altLabel xml:lang="en">Schnapps</skos:altLabel>
        <status:term_status xml:lang="en">testing</status:term_status>
        <skos:prefLabel xml:lang="ko">리큐어</skos:prefLabel>
        <rdfs:seeAlso rdf:resource="http://en.wikipedia.org/wiki/Liqueur"/>
        <rdfs:isDefinedBy rdf:resource="http://rdfs.co/bevon/"/>
    </owl:Class>
    


    <!-- http://rdfs.co/bevon/Longneck -->

    <owl:Class rdf:about="&bevon;Longneck">
        <rdfs:subClassOf rdf:resource="&bevon;BeerBottle"/>
        <dcterms:issued rdf:datatype="&xsd;date">2013-07-04+09:00</dcterms:issued>
        <dcterms:modified rdf:datatype="&xsd;date">2014-03-01+09:00</dcterms:modified>
        <skos:definition xml:lang="en">
    A longneck is a type of beer bottle with a long neck.
    </skos:definition>
        <rdfs:comment xml:lang="en">
    It is known as the standard longneck bottle or industry standard bottle
    (ISB). The ISB longnecks have a uniform capacity, height, weight and
    diameter and can be reused on average 16 times. The long neck offers a long
    cushion of air to absorb the pressure of carbonation to reduce the risk of
    exploding. The longneck also provides a handle for drinking directly from
    the bottle without transferring body heat to the beer from one&apos;s hand.
    </rdfs:comment>
        <skos:altLabel xml:lang="en">Industry Standard Bottle</skos:altLabel>
        <skos:prefLabel xml:lang="en">Longneck</skos:prefLabel>
        <skos:altLabel xml:lang="en">North American Longneck</skos:altLabel>
        <status:term_status xml:lang="en">unstable</status:term_status>
        <skos:prefLabel xml:lang="ko">긴목 맥주병</skos:prefLabel>
        <rdfs:isDefinedBy rdf:resource="http://rdfs.co/bevon/"/>
    </owl:Class>
    


    <!-- http://rdfs.co/bevon/MaltWhisky -->

    <owl:Class rdf:about="&bevon;MaltWhisky">
        <rdfs:subClassOf rdf:resource="&bevon;Whisky"/>
        <rdfs:subClassOf rdf:resource="&pto;Malt_whisky"/>
        <dcterms:issued rdf:datatype="&xsd;date">2013-07-04+09:00</dcterms:issued>
        <dcterms:modified rdf:datatype="&xsd;date">2014-03-01+09:00</dcterms:modified>
        <skos:definition xml:lang="en">
    Malt whisky is whisky that is made from a fermented mash produced primarily
    from a malted grain.
    </skos:definition>
        <skos:altLabel xml:lang="en">Malt Whiskey</skos:altLabel>
        <skos:prefLabel xml:lang="en">Malt Whisky</skos:prefLabel>
        <status:term_status xml:lang="en">unstable</status:term_status>
        <skos:prefLabel xml:lang="ko">몰트 위스키</skos:prefLabel>
        <rdfs:seeAlso rdf:resource="http://en.wikipedia.org/wiki/Malt_whisky"/>
        <rdfs:isDefinedBy rdf:resource="http://rdfs.co/bevon/"/>
    </owl:Class>
    


    <!-- http://rdfs.co/bevon/MineralWater -->

    <owl:Class rdf:about="&bevon;MineralWater">
        <rdfs:subClassOf rdf:resource="&bevon;Water"/>
        <rdfs:subClassOf rdf:resource="&pto;Mineral_water"/>
        <dcterms:issued rdf:datatype="&xsd;date">2013-07-04+09:00</dcterms:issued>
        <dcterms:modified rdf:datatype="&xsd;date">2014-03-01+09:00</dcterms:modified>
        <skos:definition xml:lang="en">
    Mineral water is water from a mineral spring containing various minerals
    such as salts and sulfur compounds.
    </skos:definition>
        <rdfs:comment xml:lang="en">
    Mineral water may be sparkling due to contained gases.
    </rdfs:comment>
        <skos:prefLabel xml:lang="en">Mineral Water</skos:prefLabel>
        <status:term_status xml:lang="en">unstable</status:term_status>
        <skos:prefLabel xml:lang="ko">광천수</skos:prefLabel>
        <rdfs:seeAlso rdf:resource="http://en.wikipedia.org/wiki/Mineral_water"/>
        <rdfs:isDefinedBy rdf:resource="http://rdfs.co/bevon/"/>
    </owl:Class>
    


    <!-- http://rdfs.co/bevon/MixedDrink -->

    <owl:Class rdf:about="&bevon;MixedDrink">
        <rdfs:subClassOf rdf:resource="&bevon;Beverage"/>
        <rdfs:subClassOf rdf:resource="&pto;Mixed_drink"/>
        <dcterms:issued rdf:datatype="&xsd;date">2013-07-04+09:00</dcterms:issued>
        <dcterms:modified rdf:datatype="&xsd;date">2014-03-01+09:00</dcterms:modified>
        <skos:definition xml:lang="en">
    A mixed drink is a beverage in which two or more ingredients are mixed.
    </skos:definition>
        <rdfs:comment xml:lang="en">
    Some mixed drinks are alcoholic beverages that contain liquor; others are
    non-alcoholic.
    </rdfs:comment>
        <skos:prefLabel xml:lang="en">Mixed Drink</skos:prefLabel>
        <status:term_status xml:lang="en">testing</status:term_status>
        <skos:prefLabel xml:lang="ko">혼합 음료</skos:prefLabel>
        <rdfs:seeAlso rdf:resource="http://en.wikipedia.org/wiki/Mixed_drink"/>
        <rdfs:isDefinedBy rdf:resource="http://rdfs.co/bevon/"/>
    </owl:Class>
    


    <!-- http://rdfs.co/bevon/Mocktail -->

    <owl:Class rdf:about="&bevon;Mocktail">
        <rdfs:subClassOf rdf:resource="&bevon;MixedDrink"/>
        <rdfs:subClassOf rdf:resource="&bevon;NonAlcoholicBeverage"/>
        <dcterms:issued rdf:datatype="&xsd;date">2013-07-04+09:00</dcterms:issued>
        <dcterms:modified rdf:datatype="&xsd;date">2014-03-01+09:00</dcterms:modified>
        <skos:definition xml:lang="en">
    Mocktails are mock cocktails, or those that do not contain any alcohol.
    </skos:definition>
        <skos:prefLabel xml:lang="en">Mocktail</skos:prefLabel>
        <status:term_status xml:lang="en">unstable</status:term_status>
        <skos:prefLabel xml:lang="ko">목테일</skos:prefLabel>
        <rdfs:isDefinedBy rdf:resource="http://rdfs.co/bevon/"/>
    </owl:Class>
    


    <!-- http://rdfs.co/bevon/NonAlcoholicBeer -->

    <owl:Class rdf:about="&bevon;NonAlcoholicBeer">
        <rdfs:subClassOf rdf:resource="&bevon;NonAlcoholicBeverage"/>
        <rdfs:subClassOf rdf:resource="&pto;Low-alcohol_beer"/>
        <dcterms:issued rdf:datatype="&xsd;date">2013-07-04+09:00</dcterms:issued>
        <dcterms:modified rdf:datatype="&xsd;date">2014-03-01+09:00</dcterms:modified>
        <skos:definition xml:lang="en">
    Non-alcohol beer (also called light beer, low-alcoholic beer, small beer,
    small ale, or near-beer) is beer with low alcohol content or no alcohol,
    which aim to reproduce the taste of beer without the inebriating effects of
    standard alcoholic brews.
    </skos:definition>
        <skos:altLabel xml:lang="en">Low-alcoholic Beer</skos:altLabel>
        <skos:prefLabel xml:lang="en">Non-alcoholic Beer</skos:prefLabel>
        <status:term_status xml:lang="en">unstable</status:term_status>
        <skos:prefLabel xml:lang="ko">비알코올 맥주</skos:prefLabel>
        <rdfs:seeAlso rdf:resource="http://en.wikipedia.org/wiki/Low-alcohol_beer"/>
        <rdfs:isDefinedBy rdf:resource="http://rdfs.co/bevon/"/>
    </owl:Class>
    


    <!-- http://rdfs.co/bevon/NonAlcoholicBeverage -->

    <owl:Class rdf:about="&bevon;NonAlcoholicBeverage">
        <rdfs:subClassOf rdf:resource="&bevon;Beverage"/>
        <rdfs:subClassOf rdf:resource="&pto;Non-alcoholic_beverage"/>
        <dcterms:issued rdf:datatype="&xsd;date">2013-07-04+09:00</dcterms:issued>
        <dcterms:modified rdf:datatype="&xsd;date">2014-03-01+09:00</dcterms:modified>
        <skos:definition xml:lang="en">
     A non-alcoholic beverage (also known as a virgin drink) is defined
     in the U.S. as a beverage that contains less than 0.5% alcohol by volume.
     </skos:definition>
        <skos:prefLabel xml:lang="en">Non-alcoholic Beverage</skos:prefLabel>
        <status:term_status xml:lang="en">testing</status:term_status>
        <skos:prefLabel xml:lang="ko">비알코올 음료</skos:prefLabel>
        <rdfs:seeAlso rdf:resource="http://en.wikipedia.org/wiki/Non-alcoholic_beverage"/>
        <rdfs:isDefinedBy rdf:resource="http://rdfs.co/bevon/"/>
    </owl:Class>
    


    <!-- http://rdfs.co/bevon/PaleAle -->

    <owl:Class rdf:about="&bevon;PaleAle">
        <rdfs:subClassOf rdf:resource="&bevon;Ale"/>
        <rdfs:subClassOf rdf:resource="&pto;Pale_ale"/>
        <dcterms:issued rdf:datatype="&xsd;date">2013-07-04+09:00</dcterms:issued>
        <dcterms:modified rdf:datatype="&xsd;date">2014-03-01+09:00</dcterms:modified>
        <rdfs:comment xml:lang="en">
    It is one of the world&apos;s major beer styles.
    </rdfs:comment>
        <skos:definition xml:lang="en">
    Pale ale is a beer made by warm fermentation using predominantly pale malt.
    </skos:definition>
        <skos:prefLabel xml:lang="en">Pale Ale</skos:prefLabel>
        <status:term_status xml:lang="en">unstable</status:term_status>
        <skos:prefLabel xml:lang="ko">페일 에일</skos:prefLabel>
        <rdfs:seeAlso rdf:resource="http://en.wikipedia.org/wiki/Pale_ale"/>
        <rdfs:isDefinedBy rdf:resource="http://rdfs.co/bevon/"/>
    </owl:Class>
    


    <!-- http://rdfs.co/bevon/PaleLager -->

    <owl:Class rdf:about="&bevon;PaleLager">
        <rdfs:subClassOf rdf:resource="&bevon;Lager"/>
        <rdfs:subClassOf rdf:resource="&pto;Pale_lager"/>
        <dcterms:issued rdf:datatype="&xsd;date">2013-07-04+09:00</dcterms:issued>
        <dcterms:modified rdf:datatype="&xsd;date">2014-03-01+09:00</dcterms:modified>
        <skos:definition xml:lang="en">
    Pale lager is a very pale to golden-colored beer with a well attenuated
    body and a varying degree of noble hop bitterness.
    </skos:definition>
        <skos:prefLabel xml:lang="en">Pale Lager</skos:prefLabel>
        <status:term_status xml:lang="en">unstable</status:term_status>
        <skos:prefLabel xml:lang="ko">페일 라거</skos:prefLabel>
        <rdfs:seeAlso rdf:resource="http://en.wikipedia.org/wiki/Pale_lager"/>
        <rdfs:isDefinedBy rdf:resource="http://rdfs.co/bevon/"/>
    </owl:Class>
    


    <!-- http://rdfs.co/bevon/Pilsner -->

    <owl:Class rdf:about="&bevon;Pilsner">
        <rdfs:subClassOf rdf:resource="&bevon;PaleLager"/>
        <rdfs:subClassOf rdf:resource="&pto;Pilsner"/>
        <dcterms:issued rdf:datatype="&xsd;date">2013-07-04+09:00</dcterms:issued>
        <dcterms:modified rdf:datatype="&xsd;date">2014-03-01+09:00</dcterms:modified>
        <rdfs:comment xml:lang="en">
    It took its name from the city of Pilsen (Plzeň, Bohemia, Czech Republic,
    where it was first produced in 1842).
    </rdfs:comment>
        <skos:definition xml:lang="en">
    Pilsner (also pilsener or simply pils) is a type of pale lager.
    </skos:definition>
        <skos:altLabel xml:lang="en">Pils</skos:altLabel>
        <skos:altLabel xml:lang="en">Pilsener</skos:altLabel>
        <skos:prefLabel xml:lang="en">Pilsner</skos:prefLabel>
        <status:term_status xml:lang="en">unstable</status:term_status>
        <skos:prefLabel xml:lang="ko">필스너</skos:prefLabel>
        <rdfs:seeAlso rdf:resource="http://en.wikipedia.org/wiki/Pilsner"/>
        <rdfs:isDefinedBy rdf:resource="http://rdfs.co/bevon/"/>
    </owl:Class>
    


    <!-- http://rdfs.co/bevon/Pisco -->

    <owl:Class rdf:about="&bevon;Pisco">
        <rdfs:subClassOf rdf:resource="&bevon;Brandy"/>
        <rdfs:subClassOf rdf:resource="&pto;Pisco"/>
        <dcterms:issued rdf:datatype="&xsd;date">2013-07-04+09:00</dcterms:issued>
        <dcterms:modified rdf:datatype="&xsd;date">2014-03-01+09:00</dcterms:modified>
        <skos:definition xml:lang="en">
    Pisco is a colorless or yellowish-to-amber colored grape brandy produced
    in winemaking regions of Peru and Chile.
    </skos:definition>
        <skos:prefLabel xml:lang="en">Pisco</skos:prefLabel>
        <status:term_status xml:lang="en">testing</status:term_status>
        <skos:prefLabel xml:lang="ko">피스코</skos:prefLabel>
        <rdfs:seeAlso rdf:resource="http://en.wikipedia.org/wiki/Pisco"/>
        <rdfs:isDefinedBy rdf:resource="http://rdfs.co/bevon/"/>
    </owl:Class>
    


    <!-- http://rdfs.co/bevon/PlasticBottle -->

    <owl:Class rdf:about="&bevon;PlasticBottle">
        <rdfs:subClassOf rdf:resource="&bevon;Container"/>
        <dcterms:issued rdf:datatype="&xsd;date">2013-07-04+09:00</dcterms:issued>
        <dcterms:modified rdf:datatype="&xsd;date">2014-03-01+09:00</dcterms:modified>
        <skos:definition xml:lang="en">
    A plastic bottle is a bottle constructed of plastic.
    </skos:definition>
        <rdfs:comment xml:lang="en">
    Plastic bottles are typically used to store liquids such as water, soft
    drinks, motor oil, cooking oil, medicine, shampoo, milk, and ink.
    </rdfs:comment>
        <skos:prefLabel xml:lang="en">Plastic Bottle</skos:prefLabel>
        <status:term_status xml:lang="en">unstable</status:term_status>
        <skos:prefLabel xml:lang="ko">플라스틱 병</skos:prefLabel>
        <rdfs:seeAlso rdf:resource="http://en.wikipedia.org/wiki/Plastic_bottle"/>
        <rdfs:isDefinedBy rdf:resource="http://rdfs.co/bevon/"/>
    </owl:Class>
    


    <!-- http://rdfs.co/bevon/Porter -->

    <owl:Class rdf:about="&bevon;Porter">
        <rdfs:subClassOf rdf:resource="&bevon;Ale"/>
        <rdfs:subClassOf rdf:resource="&pto;English_porter"/>
        <dcterms:issued rdf:datatype="&xsd;date">2013-07-04+09:00</dcterms:issued>
        <dcterms:modified rdf:datatype="&xsd;date">2014-03-01+09:00</dcterms:modified>
        <skos:definition xml:lang="en">
    Porter is a dark style of beer originating in London in the 18th century,
    descended from brown beer, a well hopped beer made from brown malt.
    </skos:definition>
        <rdfs:comment xml:lang="en">
    The name came about as a result of its popularity with street and river
    porters.
    </rdfs:comment>
        <skos:altLabel xml:lang="en">English Porter</skos:altLabel>
        <skos:prefLabel xml:lang="en">Porter</skos:prefLabel>
        <status:term_status xml:lang="en">unstable</status:term_status>
        <skos:prefLabel xml:lang="ko">포터</skos:prefLabel>
        <rdfs:seeAlso rdf:resource="http://en.wikipedia.org/wiki/English_porter"/>
        <rdfs:isDefinedBy rdf:resource="http://rdfs.co/bevon/"/>
    </owl:Class>
    


    <!-- http://rdfs.co/bevon/RedWine -->

    <owl:Class rdf:about="&bevon;RedWine">
        <rdfs:subClassOf rdf:resource="&bevon;Wine"/>
        <rdfs:subClassOf rdf:resource="&pto;Red_wine"/>
        <dcterms:modified rdf:datatype="&xsd;date">2014-03-07+09:00</dcterms:modified>
        <dcterms:issued rdf:datatype="&xsd;date">2014-03-07+09:00</dcterms:issued>
        <skos:definition xml:lang="en">
    Red wine is a type of wine made from dark-coloured (black) grape varieties.
    </skos:definition>
        <rdfs:comment xml:lang="en">
    The actual colour of the wine can range from intense violet, typical of
    young wines, through to brick red for mature wines and brown for older red
    wines.
    </rdfs:comment>
        <skos:prefLabel xml:lang="en">Red Wine</skos:prefLabel>
        <status:term_status xml:lang="en">testing</status:term_status>
        <skos:prefLabel xml:lang="fr">Vin Rouge</skos:prefLabel>
        <skos:prefLabel xml:lang="ko">레드 와인</skos:prefLabel>
        <rdfs:seeAlso rdf:resource="http://en.wikipedia.org/wiki/Red_wine"/>
        <rdfs:isDefinedBy rdf:resource="http://rdfs.co/bevon/"/>
    </owl:Class>
    


    <!-- http://rdfs.co/bevon/Rum -->

    <owl:Class rdf:about="&bevon;Rum">
        <rdfs:subClassOf rdf:resource="&bevon;DistilledBeverage"/>
        <rdfs:subClassOf rdf:resource="&pto;Rum"/>
        <dcterms:issued rdf:datatype="&xsd;date">2013-07-04+09:00</dcterms:issued>
        <dcterms:modified rdf:datatype="&xsd;date">2014-03-01+09:00</dcterms:modified>
        <skos:definition xml:lang="en">
    Rum is a distilled alcoholic beverage made from sugarcane byproducts, such
    as molasses, or directly from sugarcane juice, by a process of fermentation
    and distillation.
    </skos:definition>
        <rdfs:comment xml:lang="en">
    The distillate, a clear liquid, is then usually aged in
    oak barrels.
    </rdfs:comment>
        <skos:prefLabel xml:lang="en">Rum</skos:prefLabel>
        <status:term_status xml:lang="en">testing</status:term_status>
        <skos:prefLabel xml:lang="es">Ron</skos:prefLabel>
        <skos:prefLabel xml:lang="ko">럼</skos:prefLabel>
        <rdfs:seeAlso rdf:resource="http://en.wikipedia.org/wiki/Rum"/>
        <rdfs:isDefinedBy rdf:resource="http://rdfs.co/bevon/"/>
    </owl:Class>
    


    <!-- http://rdfs.co/bevon/Sake -->

    <owl:Class rdf:about="&bevon;Sake">
        <rdfs:subClassOf rdf:resource="&bevon;FermentedBeverage"/>
        <rdfs:subClassOf rdf:resource="&pto;Sake"/>
        <dcterms:issued rdf:datatype="&xsd;date">2013-07-04+09:00</dcterms:issued>
        <dcterms:modified rdf:datatype="&xsd;date">2014-03-01+09:00</dcterms:modified>
        <skos:definition xml:lang="en">
    Sake or saké is an alcoholic beverage of Japanese origin that is made from
    fermented rice.
    </skos:definition>
        <skos:altLabel xml:lang="en">Rice Wine</skos:altLabel>
        <skos:prefLabel xml:lang="en">Sake</skos:prefLabel>
        <status:term_status xml:lang="en">testing</status:term_status>
        <skos:prefLabel xml:lang="fr">Saké</skos:prefLabel>
        <skos:prefLabel xml:lang="ko">사케</skos:prefLabel>
        <rdfs:seeAlso rdf:resource="http://en.wikipedia.org/wiki/Sake"/>
        <rdfs:isDefinedBy rdf:resource="http://rdfs.co/bevon/"/>
    </owl:Class>
    


    <!-- http://rdfs.co/bevon/ScotchWhisky -->

    <owl:Class rdf:about="&bevon;ScotchWhisky">
        <rdfs:subClassOf rdf:resource="&bevon;Whisky"/>
        <rdfs:subClassOf rdf:resource="&pto;Scotch_whisky"/>
        <dcterms:issued rdf:datatype="&xsd;date">2013-07-04+09:00</dcterms:issued>
        <dcterms:modified rdf:datatype="&xsd;date">2014-03-01+09:00</dcterms:modified>
        <rdfs:comment xml:lang="en">
    All Scotch whisky was originally made from malt barley. Commercial
    distilleries began introducing whisky made from wheat and rye in the late
    eighteenth century.
    </rdfs:comment>
        <skos:definition xml:lang="en">
    Scotch whisky (often referred to simply as &quot;Scotch&quot;) is malt whisky or grain
    whisky made in Scotland.
    </skos:definition>
        <skos:altLabel xml:lang="en">Scotch Whiskey</skos:altLabel>
        <skos:prefLabel xml:lang="en">Scotch Whisky</skos:prefLabel>
        <status:term_status xml:lang="en">unstable</status:term_status>
        <skos:prefLabel xml:lang="ko">스카치 위스키</skos:prefLabel>
        <rdfs:seeAlso rdf:resource="http://en.wikipedia.org/wiki/Scotch_whisky"/>
        <rdfs:isDefinedBy rdf:resource="http://rdfs.co/bevon/"/>
    </owl:Class>
    


    <!-- http://rdfs.co/bevon/Shandy -->

    <owl:Class rdf:about="&bevon;Shandy">
        <rdfs:subClassOf rdf:resource="&bevon;Cocktail"/>
        <rdfs:subClassOf rdf:resource="&pto;Shandy"/>
        <dcterms:issued rdf:datatype="&xsd;date">2013-07-04+09:00</dcterms:issued>
        <dcterms:modified rdf:datatype="&xsd;date">2014-03-01+09:00</dcterms:modified>
        <skos:definition xml:lang="en">
    A shandy, or shandygaff, is beer mixed with a soft drink, carbonated
    lemonade, ginger beer, ginger ale, or apple juice.
    </skos:definition>
        <rdfs:comment xml:lang="en">
    The proportions of the two ingredients are adjusted to taste, usually
    half-and-half.
    </rdfs:comment>
        <skos:prefLabel xml:lang="en">Shandy</skos:prefLabel>
        <status:term_status xml:lang="en">unstable</status:term_status>
        <skos:prefLabel xml:lang="ko">섄디</skos:prefLabel>
        <rdfs:seeAlso rdf:resource="http://en.wikipedia.org/wiki/Shandy"/>
        <rdfs:isDefinedBy rdf:resource="http://rdfs.co/bevon/"/>
    </owl:Class>
    


    <!-- http://rdfs.co/bevon/SingleMaltScotch -->

    <owl:Class rdf:about="&bevon;SingleMaltScotch">
        <rdfs:subClassOf rdf:resource="&bevon;ScotchWhisky"/>
        <rdfs:subClassOf rdf:resource="&bevon;SingleMaltWhisky"/>
        <rdfs:subClassOf rdf:resource="&pto;Single_malt_Scotch"/>
        <dcterms:issued rdf:datatype="&xsd;date">2013-07-04+09:00</dcterms:issued>
        <dcterms:modified rdf:datatype="&xsd;date">2014-03-01+09:00</dcterms:modified>
        <rdfs:comment xml:lang="en">
    As with any Scotch whisky, a single malt Scotch must be distilled in
    Scotland and matured in oak casks in Scotland for at least three years
    (most single malts are matured longer).
    </rdfs:comment>
        <skos:definition xml:lang="en">
    Single Malt Scotch is single malt whisky made in Scotland using a pot still
    distillation process at a single distillery, with malted barley as the only
    grain ingredient.
    </skos:definition>
        <skos:prefLabel xml:lang="en">Single Malt Scotch</skos:prefLabel>
        <status:term_status xml:lang="en">unstable</status:term_status>
        <skos:prefLabel xml:lang="ko">싱글 몰트 스카치</skos:prefLabel>
        <rdfs:seeAlso rdf:resource="http://en.wikipedia.org/wiki/Single_malt_Scotch"/>
        <rdfs:isDefinedBy rdf:resource="http://rdfs.co/bevon/"/>
    </owl:Class>
    


    <!-- http://rdfs.co/bevon/SingleMaltWhisky -->

    <owl:Class rdf:about="&bevon;SingleMaltWhisky">
        <rdfs:subClassOf rdf:resource="&bevon;MaltWhisky"/>
        <rdfs:subClassOf rdf:resource="&pto;Single_malt_whisky"/>
        <dcterms:issued rdf:datatype="&xsd;date">2013-07-04+09:00</dcterms:issued>
        <dcterms:modified rdf:datatype="&xsd;date">2014-03-01+09:00</dcterms:modified>
        <skos:definition xml:lang="en">
    Single malt whisky is a whisky made at one particular distillery from a
    mash that uses only malted grain, ordinarily barley.
    </skos:definition>
        <skos:altLabel xml:lang="en">Single Malt Whiskey</skos:altLabel>
        <skos:prefLabel xml:lang="en">Single Malt Whisky</skos:prefLabel>
        <status:term_status xml:lang="en">unstable</status:term_status>
        <skos:prefLabel xml:lang="ko">싱글 몰트 위스키</skos:prefLabel>
        <rdfs:seeAlso rdf:resource="http://en.wikipedia.org/wiki/Single_malt_whisky"/>
        <rdfs:isDefinedBy rdf:resource="http://rdfs.co/bevon/"/>
    </owl:Class>
    


    <!-- http://rdfs.co/bevon/Soju -->

    <owl:Class rdf:about="&bevon;Soju">
        <rdfs:subClassOf rdf:resource="&bevon;DistilledBeverage"/>
        <rdfs:subClassOf rdf:resource="&pto;Soju"/>
        <dcterms:issued rdf:datatype="&xsd;date">2013-07-04+09:00</dcterms:issued>
        <dcterms:modified rdf:datatype="&xsd;date">2014-03-01+09:00</dcterms:modified>
        <rdfs:comment xml:lang="en">
    Its taste is comparable to vodka, though often slightly sweeter due to
    sugars added in the manufacturing process.
    </rdfs:comment>
        <skos:definition xml:lang="en">
    Soju is a distilled beverage native to Korea.
    </skos:definition>
        <skos:prefLabel xml:lang="en">Soju</skos:prefLabel>
        <status:term_status xml:lang="en">testing</status:term_status>
        <skos:prefLabel xml:lang="ko">소주</skos:prefLabel>
        <rdfs:seeAlso rdf:resource="http://en.wikipedia.org/wiki/Soju"/>
        <rdfs:isDefinedBy rdf:resource="http://rdfs.co/bevon/"/>
    </owl:Class>
    


    <!-- http://rdfs.co/bevon/SpeysideSingleMalt -->

    <owl:Class rdf:about="&bevon;SpeysideSingleMalt">
        <rdfs:subClassOf rdf:resource="&bevon;SingleMaltScotch"/>
        <rdfs:subClassOf rdf:resource="&pto;Speyside_single_malts"/>
        <dcterms:issued rdf:datatype="&xsd;date">2013-07-04+09:00</dcterms:issued>
        <dcterms:modified rdf:datatype="&xsd;date">2014-03-01+09:00</dcterms:modified>
        <skos:definition xml:lang="en">
    Speyside single malts are single malt Scotch whiskies, distilled in
    Strathspey, the area around the River Spey in Moray and Badenoch and
    Strathspey, in northeastern Scotland.
    </skos:definition>
        <skos:prefLabel xml:lang="en">Speyside Single Malt</skos:prefLabel>
        <status:term_status xml:lang="en">unstable</status:term_status>
        <skos:prefLabel xml:lang="ko">스페이사이드 싱글 몰트</skos:prefLabel>
        <rdfs:seeAlso rdf:resource="http://en.wikipedia.org/wiki/Speyside_single_malts"/>
        <rdfs:isDefinedBy rdf:resource="http://rdfs.co/bevon/"/>
    </owl:Class>
    


    <!-- http://rdfs.co/bevon/Stout -->

    <owl:Class rdf:about="&bevon;Stout">
        <rdfs:subClassOf rdf:resource="&bevon;Porter"/>
        <rdfs:subClassOf rdf:resource="&pto;Stout"/>
        <dcterms:issued rdf:datatype="&xsd;date">2013-07-04+09:00</dcterms:issued>
        <dcterms:modified rdf:datatype="&xsd;date">2014-03-01+09:00</dcterms:modified>
        <skos:definition xml:lang="en">
    Stout is a dark beer made using roasted malt or roasted barley, hops, water
    and yeast.
    </skos:definition>
        <rdfs:comment xml:lang="en">
    Stouts were traditionally the generic term for the strongest or stoutest
    porters, typically 7% or 8%, produced by a brewery.
    </rdfs:comment>
        <skos:prefLabel xml:lang="en">Stout</skos:prefLabel>
        <skos:altLabel xml:lang="en">Strong Porter</skos:altLabel>
        <status:term_status xml:lang="en">unstable</status:term_status>
        <skos:prefLabel xml:lang="ko">스타우트</skos:prefLabel>
        <rdfs:seeAlso rdf:resource="http://en.wikipedia.org/wiki/Stout"/>
        <rdfs:isDefinedBy rdf:resource="http://rdfs.co/bevon/"/>
    </owl:Class>
    


    <!-- http://rdfs.co/bevon/Tequila -->

    <owl:Class rdf:about="&bevon;Tequila">
        <rdfs:subClassOf rdf:resource="&bevon;DistilledBeverage"/>
        <rdfs:subClassOf rdf:resource="&pto;Tequila"/>
        <dcterms:issued rdf:datatype="&xsd;date">2013-07-04+09:00</dcterms:issued>
        <dcterms:modified rdf:datatype="&xsd;date">2014-03-01+09:00</dcterms:modified>
        <skos:definition xml:lang="en">
    Tequila is a distilled beverage made from the blue agave plant, primarily
    in the area surrounding the city of Tequila, 65 kilometres (40 mi)
    northwest of Guadalajara, and in the highlands (Los Altos) of the western
    Mexican state of Jalisco.
    </skos:definition>
        <skos:prefLabel xml:lang="en">Tequila</skos:prefLabel>
        <status:term_status xml:lang="en">testing</status:term_status>
        <skos:prefLabel xml:lang="ko">테킬라</skos:prefLabel>
        <rdfs:seeAlso rdf:resource="http://en.wikipedia.org/wiki/Tequila"/>
        <rdfs:isDefinedBy rdf:resource="http://rdfs.co/bevon/"/>
    </owl:Class>
    


    <!-- http://rdfs.co/bevon/TequilaBlanco -->

    <owl:Class rdf:about="&bevon;TequilaBlanco">
        <rdfs:subClassOf rdf:resource="&bevon;Tequila"/>
        <dcterms:issued rdf:datatype="&xsd;date">2013-07-04+09:00</dcterms:issued>
        <dcterms:modified rdf:datatype="&xsd;date">2014-03-01+09:00</dcterms:modified>
        <skos:definition xml:lang="en">
    Tequila Blanco (&quot;white&quot;) or Plata (&quot;silver&quot;) is a white spirit, un-aged and
    bottled or stored immediately after distillation, or aged less than two
    months in stainless steel or neutral oak barrels.
    </skos:definition>
        <skos:prefLabel xml:lang="en">Tequila Blanco</skos:prefLabel>
        <skos:altLabel xml:lang="en">Tequila Plata</skos:altLabel>
        <status:term_status xml:lang="en">unstable</status:term_status>
        <skos:prefLabel xml:lang="ko">테킬라 블랑코</skos:prefLabel>
        <rdfs:isDefinedBy rdf:resource="http://rdfs.co/bevon/"/>
    </owl:Class>
    


    <!-- http://rdfs.co/bevon/Vodka -->

    <owl:Class rdf:about="&bevon;Vodka">
        <rdfs:subClassOf rdf:resource="&bevon;DistilledBeverage"/>
        <rdfs:subClassOf rdf:resource="&pto;Vodka"/>
        <dcterms:issued rdf:datatype="&xsd;date">2013-07-04+09:00</dcterms:issued>
        <dcterms:modified rdf:datatype="&xsd;date">2014-03-01+09:00</dcterms:modified>
        <skos:definition xml:lang="en">
    Vodka is a distilled beverage composed primarily of water and ethanol,
    sometimes with traces of impurities and flavorings.
    </skos:definition>
        <rdfs:comment xml:lang="en">
    Vodka is made by the distillation of fermented substances such as grains,
    potatoes, or sometimes fruits or sugar.
    </rdfs:comment>
        <skos:prefLabel xml:lang="en">Vodka</skos:prefLabel>
        <status:term_status xml:lang="en">testing</status:term_status>
        <skos:prefLabel xml:lang="ko">보드카</skos:prefLabel>
        <skos:prefLabel xml:lang="pl">Wódka</skos:prefLabel>
        <skos:prefLabel xml:lang="ru">водка</skos:prefLabel>
        <rdfs:seeAlso rdf:resource="http://en.wikipedia.org/wiki/Vodka"/>
        <rdfs:isDefinedBy rdf:resource="http://rdfs.co/bevon/"/>
    </owl:Class>
    


    <!-- http://rdfs.co/bevon/Water -->

    <owl:Class rdf:about="&bevon;Water">
        <rdfs:subClassOf rdf:resource="&bevon;NonAlcoholicBeverage"/>
        <rdfs:subClassOf rdf:resource="&pto;Water"/>
        <dcterms:issued rdf:datatype="&xsd;date">2013-07-04+09:00</dcterms:issued>
        <dcterms:modified rdf:datatype="&xsd;date">2014-03-01+09:00</dcterms:modified>
        <skos:definition xml:lang="en">
    In the Beverage Ontology, Water means a drinking water.
    </skos:definition>
        <skos:prefLabel xml:lang="en">Water</skos:prefLabel>
        <status:term_status xml:lang="en">testing</status:term_status>
        <skos:prefLabel xml:lang="ko">물</skos:prefLabel>
        <rdfs:seeAlso rdf:resource="http://en.wikipedia.org/wiki/Water"/>
        <rdfs:isDefinedBy rdf:resource="http://rdfs.co/bevon/"/>
    </owl:Class>
    


    <!-- http://rdfs.co/bevon/Whisky -->

    <owl:Class rdf:about="&bevon;Whisky">
        <rdfs:subClassOf rdf:resource="&bevon;DistilledBeverage"/>
        <rdfs:subClassOf rdf:resource="&pto;Whisky"/>
        <dcterms:issued rdf:datatype="&xsd;date">2013-07-04+09:00</dcterms:issued>
        <dcterms:modified rdf:datatype="&xsd;date">2014-03-01+09:00</dcterms:modified>
        <rdfs:comment xml:lang="en">
    Different grains are used for different varieties, including barley, malted
    barley, rye, malted rye, wheat, and corn. Whisky is typically aged in
    wooden casks, made generally of charred white oak.
    </rdfs:comment>
        <skos:definition xml:lang="en">
    Whisky or whiskey is a type of distilled alcoholic beverage made from
    fermented grain mash.
    </skos:definition>
        <skos:altLabel xml:lang="en">Whiskey</skos:altLabel>
        <skos:prefLabel xml:lang="en">Whisky</skos:prefLabel>
        <status:term_status xml:lang="en">testing</status:term_status>
        <skos:prefLabel xml:lang="en">위스키</skos:prefLabel>
        <rdfs:seeAlso rdf:resource="http://en.wikipedia.org/wiki/Whisky"/>
        <rdfs:isDefinedBy rdf:resource="http://rdfs.co/bevon/"/>
    </owl:Class>
    


    <!-- http://rdfs.co/bevon/WhiteWine -->

    <owl:Class rdf:about="&bevon;WhiteWine">
        <rdfs:subClassOf rdf:resource="&bevon;Wine"/>
        <rdfs:subClassOf rdf:resource="&pto;White_wine"/>
        <dcterms:issued rdf:datatype="&xsd;date">2014-03-07+09:00</dcterms:issued>
        <dcterms:modified rdf:datatype="&xsd;date">2014-03-07+09:00</dcterms:modified>
        <rdfs:comment xml:lang="en">
    It is produced by the alcoholic fermentation of the non-coloured pulp of
    grapes which may have a white or black skin. It is treated so as to
    maintain a yellow transparent colour in the final product.
    </rdfs:comment>
        <skos:definition xml:lang="en">
    White wine is a wine whose colour can be straw-yellow, yellow-green, or
    yellow-gold coloured.
    </skos:definition>
        <skos:prefLabel xml:lang="en">White Wine</skos:prefLabel>
        <status:term_status xml:lang="en">testing</status:term_status>
        <skos:prefLabel xml:lang="fr">Vin Blanc</skos:prefLabel>
        <skos:prefLabel xml:lang="ko">화이트 와인</skos:prefLabel>
        <rdfs:seeAlso rdf:resource="http://en.wikipedia.org/wiki/White_wine"/>
        <rdfs:isDefinedBy rdf:resource="http://rdfs.co/bevon/"/>
    </owl:Class>
    


    <!-- http://rdfs.co/bevon/Wine -->

    <owl:Class rdf:about="&bevon;Wine">
        <rdfs:subClassOf rdf:resource="&bevon;FermentedBeverage"/>
        <rdfs:subClassOf rdf:resource="&pto;Wine"/>
        <dcterms:issued rdf:datatype="&xsd;date">2013-07-04+09:00</dcterms:issued>
        <dcterms:modified rdf:datatype="&xsd;date">2014-03-07+09:00</dcterms:modified>
        <skos:definition xml:lang="en">
    Wine is an alcoholic beverage made from fermented grapes or other fruits.
    </skos:definition>
        <skos:prefLabel xml:lang="en">Wine</skos:prefLabel>
        <status:term_status xml:lang="en">testing</status:term_status>
        <skos:prefLabel xml:lang="fr">Vin</skos:prefLabel>
        <skos:prefLabel xml:lang="ko">와인</skos:prefLabel>
        <rdfs:seeAlso rdf:resource="http://en.wikipedia.org/wiki/Wine"/>
        <rdfs:isDefinedBy rdf:resource="http://rdfs.co/bevon/"/>
        <skos:historyNote>
            <rdf:Description>
                <dcterms:creator rdf:resource="http://jayg.me/"/>
            </rdf:Description>
        </skos:historyNote>
    </owl:Class>
    


    <!-- http://www.productontology.org/id/Alcoholic_beverage -->

    <owl:Class rdf:about="&pto;Alcoholic_beverage"/>
    


    <!-- http://www.productontology.org/id/Ale -->

    <owl:Class rdf:about="&pto;Ale"/>
    


    <!-- http://www.productontology.org/id/American_whiskey -->

    <owl:Class rdf:about="&pto;American_whiskey"/>
    


    <!-- http://www.productontology.org/id/Beer -->

    <owl:Class rdf:about="&pto;Beer"/>
    


    <!-- http://www.productontology.org/id/Beer_cocktail -->

    <owl:Class rdf:about="&pto;Beer_cocktail"/>
    


    <!-- http://www.productontology.org/id/Bourbon_whiskey -->

    <owl:Class rdf:about="&pto;Bourbon_whiskey"/>
    


    <!-- http://www.productontology.org/id/Brandy -->

    <owl:Class rdf:about="&pto;Brandy"/>
    


    <!-- http://www.productontology.org/id/Canadian_whisky -->

    <owl:Class rdf:about="&pto;Canadian_whisky"/>
    


    <!-- http://www.productontology.org/id/Carbonated_water -->

    <owl:Class rdf:about="&pto;Carbonated_water"/>
    


    <!-- http://www.productontology.org/id/Cocktail -->

    <owl:Class rdf:about="&pto;Cocktail"/>
    


    <!-- http://www.productontology.org/id/Cognac -->

    <owl:Class rdf:about="&pto;Cognac"/>
    


    <!-- http://www.productontology.org/id/Distilled_beverage -->

    <owl:Class rdf:about="&pto;Distilled_beverage"/>
    


    <!-- http://www.productontology.org/id/Drink -->

    <owl:Class rdf:about="&pto;Drink"/>
    


    <!-- http://www.productontology.org/id/Dunkel -->

    <owl:Class rdf:about="&pto;Dunkel"/>
    


    <!-- http://www.productontology.org/id/English_porter -->

    <owl:Class rdf:about="&pto;English_porter"/>
    


    <!-- http://www.productontology.org/id/Fruit_wine -->

    <owl:Class rdf:about="&pto;Fruit_wine"/>
    


    <!-- http://www.productontology.org/id/Gin -->

    <owl:Class rdf:about="&pto;Gin"/>
    


    <!-- http://www.productontology.org/id/Highball -->

    <owl:Class rdf:about="&pto;Highball"/>
    


    <!-- http://www.productontology.org/id/Irish_whiskey -->

    <owl:Class rdf:about="&pto;Irish_whiskey"/>
    


    <!-- http://www.productontology.org/id/Japanese_whisky -->

    <owl:Class rdf:about="&pto;Japanese_whisky"/>
    


    <!-- http://www.productontology.org/id/Lager -->

    <owl:Class rdf:about="&pto;Lager"/>
    


    <!-- http://www.productontology.org/id/Liqueur -->

    <owl:Class rdf:about="&pto;Liqueur"/>
    


    <!-- http://www.productontology.org/id/Low-alcohol_beer -->

    <owl:Class rdf:about="&pto;Low-alcohol_beer"/>
    


    <!-- http://www.productontology.org/id/Malt_whisky -->

    <owl:Class rdf:about="&pto;Malt_whisky"/>
    


    <!-- http://www.productontology.org/id/Mineral_water -->

    <owl:Class rdf:about="&pto;Mineral_water"/>
    


    <!-- http://www.productontology.org/id/Mixed_drink -->

    <owl:Class rdf:about="&pto;Mixed_drink"/>
    


    <!-- http://www.productontology.org/id/Non-alcoholic_beverage -->

    <owl:Class rdf:about="&pto;Non-alcoholic_beverage"/>
    


    <!-- http://www.productontology.org/id/Pale_ale -->

    <owl:Class rdf:about="&pto;Pale_ale"/>
    


    <!-- http://www.productontology.org/id/Pale_lager -->

    <owl:Class rdf:about="&pto;Pale_lager"/>
    


    <!-- http://www.productontology.org/id/Pilsner -->

    <owl:Class rdf:about="&pto;Pilsner"/>
    


    <!-- http://www.productontology.org/id/Pisco -->

    <owl:Class rdf:about="&pto;Pisco"/>
    


    <!-- http://www.productontology.org/id/Red_wine -->

    <owl:Class rdf:about="&pto;Red_wine"/>
    


    <!-- http://www.productontology.org/id/Rum -->

    <owl:Class rdf:about="&pto;Rum"/>
    


    <!-- http://www.productontology.org/id/Sake -->

    <owl:Class rdf:about="&pto;Sake"/>
    


    <!-- http://www.productontology.org/id/Scotch_whisky -->

    <owl:Class rdf:about="&pto;Scotch_whisky"/>
    


    <!-- http://www.productontology.org/id/Shandy -->

    <owl:Class rdf:about="&pto;Shandy"/>
    


    <!-- http://www.productontology.org/id/Single_malt_Scotch -->

    <owl:Class rdf:about="&pto;Single_malt_Scotch"/>
    


    <!-- http://www.productontology.org/id/Single_malt_whisky -->

    <owl:Class rdf:about="&pto;Single_malt_whisky"/>
    


    <!-- http://www.productontology.org/id/Soju -->

    <owl:Class rdf:about="&pto;Soju"/>
    


    <!-- http://www.productontology.org/id/Speyside_single_malts -->

    <owl:Class rdf:about="&pto;Speyside_single_malts"/>
    


    <!-- http://www.productontology.org/id/Stout -->

    <owl:Class rdf:about="&pto;Stout"/>
    


    <!-- http://www.productontology.org/id/Tequila -->

    <owl:Class rdf:about="&pto;Tequila"/>
    


    <!-- http://www.productontology.org/id/Vodka -->

    <owl:Class rdf:about="&pto;Vodka"/>
    


    <!-- http://www.productontology.org/id/Water -->

    <owl:Class rdf:about="&pto;Water"/>
    


    <!-- http://www.productontology.org/id/Whisky -->

    <owl:Class rdf:about="&pto;Whisky"/>
    


    <!-- http://www.productontology.org/id/White_wine -->

    <owl:Class rdf:about="&pto;White_wine"/>
    


    <!-- http://www.productontology.org/id/Wine -->

    <owl:Class rdf:about="&pto;Wine"/>
    


    <!-- http://www.w3.org/1999/02/22-rdf-syntax-ns#Bag -->

    <owl:Class rdf:about="&rdf;Bag"/>
    


    <!-- http://www.w3.org/2006/time#DurationDescription -->

    <owl:Class rdf:about="&time;DurationDescription"/>
    


    <!-- http://www.w3.org/TR/2003/PR-owl-guide-20031209/food#PotableLiquid -->

    <owl:Class rdf:about="&fowl;PotableLiquid"/>
    


    <!-- http://www.w3.org/TR/2003/PR-owl-guide-20031209/wine#Wine -->

    <owl:Class rdf:about="&wine;Wine">
        <rdfs:subClassOf rdf:resource="&bevon;Wine"/>
    </owl:Class>
    


    <!-- http://www.w3.org/ns/adms#SemanticAsset -->

    <owl:Class rdf:about="&adms;SemanticAsset"/>
    


    <!-- http://xmlns.com/foaf/0.1/Agent -->

    <owl:Class rdf:about="&foaf;Agent"/>
    


    <!-- http://xmlns.com/foaf/0.1/Organization -->

    <owl:Class rdf:about="&foaf;Organization"/>
    


    <!-- http://xmlns.com/foaf/0.1/Person -->

    <owl:Class rdf:about="&foaf;Person"/>
    


    <!-- 
    ///////////////////////////////////////////////////////////////////////////////////////
    //
    // Individuals
    //
    ///////////////////////////////////////////////////////////////////////////////////////
     -->

    


    <!-- http://dbpedia.org/resource/Agave -->

    <owl:NamedIndividual rdf:about="http://dbpedia.org/resource/Agave"/>
    


    <!-- http://dbpedia.org/resource/Barley -->

    <owl:NamedIndividual rdf:about="http://dbpedia.org/resource/Barley"/>
    


    <!-- http://dbpedia.org/resource/Bourbon_whiskey -->

    <owl:NamedIndividual rdf:about="http://dbpedia.org/resource/Bourbon_whiskey"/>
    


    <!-- http://dbpedia.org/resource/Carbonated_water -->

    <owl:NamedIndividual rdf:about="http://dbpedia.org/resource/Carbonated_water">
        <owl:sameAs>
            <rdf:Description>
                <rdf:type rdf:resource="&bevon;CarbonatedWater"/>
                <dcterms:title xml:lang="en">Carbonated Water</dcterms:title>
            </rdf:Description>
        </owl:sameAs>
    </owl:NamedIndividual>
    


    <!-- http://dbpedia.org/resource/Chum-Churum -->

    <owl:NamedIndividual rdf:about="http://dbpedia.org/resource/Chum-Churum">
        <owl:sameAs rdf:resource="&bevon;beverage/Chum-Churum"/>
    </owl:NamedIndividual>
    


    <!-- http://dbpedia.org/resource/Diageo -->

    <owl:NamedIndividual rdf:about="http://dbpedia.org/resource/Diageo"/>
    


    <!-- http://dbpedia.org/resource/Dublin -->

    <owl:NamedIndividual rdf:about="http://dbpedia.org/resource/Dublin"/>
    


    <!-- http://dbpedia.org/resource/Glenfiddich_distillery -->

    <owl:NamedIndividual rdf:about="http://dbpedia.org/resource/Glenfiddich_distillery">
        <owl:sameAs>
            <rdf:Description>
                <rdf:type rdf:resource="&bevon;Distillery"/>
                <whisky:region rdf:resource="http://dbpedia.org/resource/Strathspey,_Scotland"/>
                <whisky:owner rdf:resource="http://dbpedia.org/resource/William_Grant_%26_Sons"/>
                <whisky:waterSource>
                    <rdf:Description>
                        <rdf:type rdf:resource="&whisky;WaterSource"/>
                        <dcterms:title xml:lang="en">Robbie Dhu Springs</dcterms:title>
                        <dcterms:title xml:lang="ko">로비 듀 수원지</dcterms:title>
                    </rdf:Description>
                </whisky:waterSource>
            </rdf:Description>
        </owl:sameAs>
    </owl:NamedIndividual>
    


    <!-- http://dbpedia.org/resource/Guinness -->

    <owl:NamedIndividual rdf:about="http://dbpedia.org/resource/Guinness">
        <owl:sameAs rdf:resource="&bevon;beverage/Guinness"/>
    </owl:NamedIndividual>
    


    <!-- http://dbpedia.org/resource/Jinro -->

    <owl:NamedIndividual rdf:about="http://dbpedia.org/resource/Jinro"/>
    


    <!-- http://dbpedia.org/resource/Kilkenny -->

    <owl:NamedIndividual rdf:about="http://dbpedia.org/resource/Kilkenny"/>
    


    <!-- http://dbpedia.org/resource/Mexico -->

    <owl:NamedIndividual rdf:about="http://dbpedia.org/resource/Mexico"/>
    


    <!-- http://dbpedia.org/resource/Oak -->

    <owl:NamedIndividual rdf:about="http://dbpedia.org/resource/Oak"/>
    


    <!-- http://dbpedia.org/resource/Qingdao -->

    <owl:NamedIndividual rdf:about="http://dbpedia.org/resource/Qingdao"/>
    


    <!-- http://dbpedia.org/resource/SABMiller -->

    <owl:NamedIndividual rdf:about="http://dbpedia.org/resource/SABMiller"/>
    


    <!-- http://dbpedia.org/resource/Sherry -->

    <owl:NamedIndividual rdf:about="http://dbpedia.org/resource/Sherry"/>
    


    <!-- http://dbpedia.org/resource/South_Korea -->

    <owl:NamedIndividual rdf:about="http://dbpedia.org/resource/South_Korea"/>
    


    <!-- http://dbpedia.org/resource/Tsingtao_Brewery -->

    <owl:NamedIndividual rdf:about="http://dbpedia.org/resource/Tsingtao_Brewery"/>
    


    <!-- http://dbpedia.org/resource/United_States -->

    <owl:NamedIndividual rdf:about="http://dbpedia.org/resource/United_States"/>
    


    <!-- http://dbpedia.org/resource/Velké_Popovice -->

    <owl:NamedIndividual rdf:about="http://dbpedia.org/resource/Velké_Popovice"/>
    


    <!-- http://dbpedia.org/resource/Whisky -->

    <owl:NamedIndividual rdf:about="http://dbpedia.org/resource/Whisky">
        <owl:sameAs>
            <rdf:Description>
                <rdf:type rdf:resource="&bevon;Whisky"/>
                <dcterms:title xml:lang="en">Whisky</dcterms:title>
            </rdf:Description>
        </owl:sameAs>
    </owl:NamedIndividual>
    


    <!-- http://dbpedia.org/resource/Anheuser–Busch_InBev -->

    <owl:NamedIndividual rdf:about="http://dbpedia.org/resource/Anheuser–Busch_InBev"/>
    


    <!-- http://dbpedia.org/resource/Clear_(color) -->

    <owl:NamedIndividual rdf:about="http://dbpedia.org/resource/Clear_(color)">
        <owl:sameAs>
            <rdf:Description>
                <rdf:type rdf:resource="&dbpedia;Colour"/>
                <dcterms:title xml:lang="en">Clear</dcterms:title>
            </rdf:Description>
        </owl:sameAs>
        <owl:sameAs>
            <rdf:Description>
                <rdf:type rdf:resource="&dbpedia;Colour"/>
                <dcterms:title xml:lang="en">Clear</dcterms:title>
            </rdf:Description>
        </owl:sameAs>
        <owl:sameAs>
            <rdf:Description>
                <rdf:type rdf:resource="&dbpedia;Colour"/>
                <dcterms:title xml:lang="en">Clear</dcterms:title>
            </rdf:Description>
        </owl:sameAs>
    </owl:NamedIndividual>
    


    <!-- http://dbpedia.org/resource/Gold_(color) -->

    <owl:NamedIndividual rdf:about="http://dbpedia.org/resource/Gold_(color)">
        <owl:sameAs>
            <rdf:Description>
                <rdf:type rdf:resource="&dbpedia;Colour"/>
                <dcterms:title xml:lang="en">Gold</dcterms:title>
            </rdf:Description>
        </owl:sameAs>
    </owl:NamedIndividual>
    


    <!-- http://dbpedia.org/resource/Kilkenny_(beer) -->

    <owl:NamedIndividual rdf:about="http://dbpedia.org/resource/Kilkenny_(beer)">
        <owl:sameAs rdf:resource="&bevon;beverage/Kilkenny"/>
    </owl:NamedIndividual>
    


    <!-- http://dbpedia.org/resource/Ruby_(color)__Ruby_Red__1 -->

    <owl:NamedIndividual rdf:about="http://dbpedia.org/resource/Ruby_(color)__Ruby_Red__1">
        <owl:sameAs>
            <rdf:Description>
                <rdf:type rdf:resource="&dbpedia;Colour"/>
                <dcterms:title xml:lang="en">Ruby Red</dcterms:title>
            </rdf:Description>
        </owl:sameAs>
    </owl:NamedIndividual>
    


    <!-- http://dbpedia.org/resource/Smithwick%27s -->

    <owl:NamedIndividual rdf:about="http://dbpedia.org/resource/Smithwick%27s">
        <owl:sameAs rdf:resource="&bevon;beverage/Smithwicks"/>
    </owl:NamedIndividual>
    


    <!-- http://dbpedia.org/resource/Strathspey,_Scotland -->

    <owl:NamedIndividual rdf:about="http://dbpedia.org/resource/Strathspey,_Scotland"/>
    


    <!-- http://dbpedia.org/resource/William_Grant_%26_Sons -->

    <owl:NamedIndividual rdf:about="http://dbpedia.org/resource/William_Grant_%26_Sons"/>
    


    <!-- http://jayg.me/ -->

    <owl:NamedIndividual rdf:about="http://jayg.me/">
        <rdf:type rdf:resource="&foaf;Person"/>
        <foaf:mbox_sha1sum>a637717b7e34b83694018e8fdd3ff334fffcd4f3</foaf:mbox_sha1sum>
        <foaf:name xml:lang="en">James G. Kim</foaf:name>
        <foaf:name xml:lang="ko">김보람</foaf:name>
        <foaf:homepage rdf:resource="http://jayg.org/"/>
    </owl:NamedIndividual>
    


    <!-- http://purl.org/colors/rgb/FFD700 -->

    <owl:NamedIndividual rdf:about="http://purl.org/colors/rgb/FFD700">
        <owl:sameAs>
            <rdf:Description>
                <rdf:type rdf:resource="&dbpedia;Colour"/>
                <dcterms:title xml:lang="en">Gold</dcterms:title>
            </rdf:Description>
        </owl:sameAs>
    </owl:NamedIndividual>
    


    <!-- http://purl.org/colors/rgb/9B111E -->

    <owl:NamedIndividual rdf:about="http://purl.org/colors/rgb/9B111E">
        <owl:sameAs>
            <rdf:Description>
                <rdf:type rdf:resource="&dbpedia;Colour"/>
                <dcterms:title xml:lang="en">Ruby Red</dcterms:title>
            </rdf:Description>
        </owl:sameAs>
    </owl:NamedIndividual>
    


    <!-- http://purl.org/vocab/whisky/terms/Whiskey -->

    <owl:NamedIndividual rdf:about="&whisky;Whiskey">
        <owl:sameAs rdf:resource="&bevon;Whisky"/>
    </owl:NamedIndividual>
    


    <!-- http://rdfs.co/bevon/BeerGroup -->

    <owl:NamedIndividual rdf:about="&bevon;BeerGroup">
        <rdf:type rdf:resource="&rdf;Bag"/>
        <rdfs:label xml:lang="en">Beer Terms</rdfs:label>
        <rdfs:comment xml:lang="en">
    In addition to the BEVON core terms, there are a number of terms for use
    when describing beverages categorized under Beer.
    </rdfs:comment>
    </owl:NamedIndividual>
    


    <!-- http://rdfs.co/bevon/CocktailGroup -->

    <owl:NamedIndividual rdf:about="&bevon;CocktailGroup">
        <rdf:type rdf:resource="&rdf;Bag"/>
        <rdfs:label xml:lang="en">Cocktail Terms</rdfs:label>
        <rdfs:comment xml:lang="en">
    These classes and properties are for describing beverages categorized under
    Mixed Drink.
    </rdfs:comment>
    </owl:NamedIndividual>
    


    <!-- http://rdfs.co/bevon/ContainerGroup -->

    <owl:NamedIndividual rdf:about="&bevon;ContainerGroup">
        <rdf:type rdf:resource="&rdf;Bag"/>
        <rdfs:label xml:lang="en">Container Terms</rdfs:label>
        <rdfs:comment xml:lang="en">
    These classes and properties are used to describe beverage containers.
    </rdfs:comment>
    </owl:NamedIndividual>
    


    <!-- http://rdfs.co/bevon/CoreGroup -->

    <owl:NamedIndividual rdf:about="&bevon;CoreGroup">
        <rdf:type rdf:resource="&rdf;Bag"/>
        <rdfs:label xml:lang="en">Core Terms</rdfs:label>
        <rdfs:comment xml:lang="en">
    These classes and properties form the core of BEVON. They describe
    characteristics of beverages in relatively broad terms.
    </rdfs:comment>
    </owl:NamedIndividual>
    


    <!-- http://rdfs.co/bevon/RedWine -->

    <owl:NamedIndividual rdf:about="&bevon;RedWine">
        <owl:sameAs rdf:resource="&wine;RedWine"/>
    </owl:NamedIndividual>
    


    <!-- http://rdfs.co/bevon/RelationGroup -->

    <owl:NamedIndividual rdf:about="&bevon;RelationGroup">
        <rdf:type rdf:resource="&rdf;Bag"/>
        <rdfs:label xml:lang="en">Relation Terms</rdfs:label>
        <rdfs:comment xml:lang="en">
    These properties are used for describing relations between beverages.
    </rdfs:comment>
    </owl:NamedIndividual>
    


    <!-- http://rdfs.co/bevon/Whisky -->

    <owl:NamedIndividual rdf:about="&bevon;Whisky"/>
    


    <!-- http://rdfs.co/bevon/WhiskyGroup -->

    <owl:NamedIndividual rdf:about="&bevon;WhiskyGroup">
        <rdf:type rdf:resource="&rdf;Bag"/>
        <rdfs:label xml:lang="en">Whisky Terms</rdfs:label>
        <rdfs:comment xml:lang="en">
    These classes describe types of whiskies.
    </rdfs:comment>
    </owl:NamedIndividual>
    


    <!-- http://rdfs.co/bevon/WhiteWine -->

    <owl:NamedIndividual rdf:about="&bevon;WhiteWine">
        <owl:sameAs rdf:resource="&wine;WhiteWine"/>
    </owl:NamedIndividual>
    


    <!-- http://rdfs.co/bevon/WineGroup -->

    <owl:NamedIndividual rdf:about="&bevon;WineGroup">
        <rdf:type rdf:resource="&rdf;Bag"/>
        <rdfs:label xml:lang="en">Wine Terms</rdfs:label>
        <rdfs:comment xml:lang="en">
    These classes describe types of wines.
    </rdfs:comment>
    </owl:NamedIndividual>
    


    <!-- http://rdfs.co/bevon/0.7 -->

    <owl:NamedIndividual rdf:about="&bevon;0.7">
        <rdf:type rdf:resource="&cc;Work"/>
        <rdf:type rdf:resource="&adms;SemanticAsset"/>
        <dcterms:description xml:lang="en">
    Beverage Ontology is a Web vocabulary for describing beverages, mainly
    alcoholic.
    </dcterms:description>
        <dcterms:title xml:lang="en">BEVON: Beverage Ontology</dcterms:title>
    </owl:NamedIndividual>
    


    <!-- http://rdfs.co/bevon/beverage/Budweiser -->

    <owl:NamedIndividual rdf:about="&bevon;beverage/Budweiser">
        <rdf:type rdf:resource="&gr;ProductOrServiceModel"/>
        <rdf:type rdf:resource="&bevon;PaleLager"/>
        <bevon:ibu rdf:datatype="&xsd;nonNegativeInteger">12</bevon:ibu>
        <bevon:launch rdf:datatype="&xsd;gYear">1876</bevon:launch>
        <bevon:srm rdf:datatype="&xsd;nonNegativeInteger">3</bevon:srm>
        <bevon:abv rdf:datatype="&xsd;decimal">5</bevon:abv>
        <bevon:description xml:lang="en">
    Budweiser is a pale lager produced by Anheuser–Busch InBev. Introduced in
    1876 by Adolphus Busch it has grown to become one of the highest selling
    beers in the United States, and is available in over 80 markets worldwide.
    </bevon:description>
        <bevon:name xml:lang="en">Budweiser</bevon:name>
        <bevon:name xml:lang="ko">버드와이저</bevon:name>
        <bevon:fermentation_base rdf:resource="http://dbpedia.org/resource/Barley"/>
        <bevon:origin rdf:resource="http://dbpedia.org/resource/United_States"/>
        <bevon:manufacturer rdf:resource="http://dbpedia.org/resource/Anheuser–Busch_InBev"/>
        <bevon:container rdf:resource="&bevon;container/330mlLongneck"/>
        <bevon:container rdf:resource="&bevon;container/355mlBeverageCan"/>
        <bevon:container rdf:resource="&bevon;container/500mlBeverageCan"/>
        <rdfs:seeAlso rdf:resource="https://en.wikipedia.org/wiki/Budweiser_(Anheuser-Busch)"/>
    </owl:NamedIndividual>
    


    <!-- http://rdfs.co/bevon/beverage/Chamisul -->

    <owl:NamedIndividual rdf:about="&bevon;beverage/Chamisul">
        <rdf:type rdf:resource="&gr;ProductOrServiceModel"/>
        <rdf:type rdf:resource="&bevon;DilutedSoju"/>
        <bevon:abv rdf:datatype="&xsd;decimal">19</bevon:abv>
        <bevon:launch rdf:datatype="&xsd;gYear">1998</bevon:launch>
        <bevon:description xml:lang="en">
    Chamisul is the diluted soju produced by HITEJiro.
    </bevon:description>
        <bevon:name xml:lang="en">Chamisul</bevon:name>
        <bevon:name xml:lang="ko">참이슬</bevon:name>
        <bevon:manufacturer rdf:resource="http://dbpedia.org/resource/Jinro"/>
        <bevon:origin rdf:resource="http://dbpedia.org/resource/South_Korea"/>
        <rdfs:seeAlso rdf:resource="http://ko.wikipedia.org/wiki/참이슬"/>
        <bevon:container rdf:resource="&bevon;container/1_8lPlasticBottle"/>
        <bevon:container rdf:resource="&bevon;container/200mlPlasticBottle"/>
        <bevon:container rdf:resource="&bevon;container/360mlGlassBottle"/>
        <bevon:container rdf:resource="&bevon;container/640mlPlasticBottle"/>
        <bevon:color>
            <rdf:Description>
                <rdf:type rdf:resource="&dbpedia;Colour"/>
                <dcterms:title xml:lang="en">Clear</dcterms:title>
            </rdf:Description>
        </bevon:color>
    </owl:NamedIndividual>
    


    <!-- http://rdfs.co/bevon/beverage/Chum-Churum -->

    <owl:NamedIndividual rdf:about="&bevon;beverage/Chum-Churum">
        <rdf:type rdf:resource="&gr;ProductOrServiceModel"/>
        <rdf:type rdf:resource="&bevon;DilutedSoju"/>
        <bevon:abv rdf:datatype="&xsd;decimal">19.5</bevon:abv>
        <bevon:launch rdf:datatype="&xsd;gYear">2006</bevon:launch>
        <bevon:description xml:lang="en">
    Chum-Churum is the diluted soju produced by Lotte Liquor.
    </bevon:description>
        <bevon:name xml:lang="en">Chum-Churum</bevon:name>
        <bevon:name xml:lang="ko">처음처럼</bevon:name>
        <bevon:origin rdf:resource="http://dbpedia.org/resource/South_Korea"/>
        <rdfs:seeAlso rdf:resource="http://ko.wikipedia.org/wiki/처음처럼_(주류)"/>
        <bevon:container rdf:resource="&bevon;container/1_8lPlasticBottle"/>
        <bevon:container rdf:resource="&bevon;container/200mlPlasticBottle"/>
        <bevon:container rdf:resource="&bevon;container/360mlGlassBottle"/>
        <bevon:container rdf:resource="&bevon;container/360mlPlasticBottle"/>
        <bevon:container rdf:resource="&bevon;container/640mlPlasticBottle"/>
        <bevon:color>
            <rdf:Description>
                <rdf:type rdf:resource="&dbpedia;Colour"/>
                <dcterms:title xml:lang="en">Clear</dcterms:title>
            </rdf:Description>
        </bevon:color>
        <bevon:manufacturer>
            <rdf:Description>
                <rdf:type rdf:resource="&foaf;Organization"/>
                <foaf:name xml:lang="en">Lotte Liquor</foaf:name>
                <foaf:name xml:lang="ko">롯데주류</foaf:name>
                <foaf:homepage rdf:resource="http://www.lotteliquor.com"/>
                <rdfs:seeAlso rdf:resource="http://ko.wikipedia.org/wiki/롯데칠성음료"/>
            </rdf:Description>
        </bevon:manufacturer>
    </owl:NamedIndividual>
    


    <!-- http://rdfs.co/bevon/beverage/DonJulioBlanco -->

    <owl:NamedIndividual rdf:about="&bevon;beverage/DonJulioBlanco">
        <rdf:type rdf:resource="&gr;ProductOrServiceModel"/>
        <rdf:type rdf:resource="&bevon;TequilaBlanco"/>
        <bevon:launch rdf:datatype="&xsd;gYear">1942</bevon:launch>
        <bevon:abv rdf:datatype="&xsd;decimal">40</bevon:abv>
        <bevon:proof rdf:datatype="&xsd;decimal">80</bevon:proof>
        <bevon:description xml:lang="en">
    Tequila Don Julio Blanco is the base from which all of our other variants
    are derived. Commonly referred to as &quot;silver&quot; tequila, its crisp agave
    flavor and hints of citrus make it an essential component to a variety of
    innovative drinks including margaritas. It can also be enjoyed neat or on
    the rocks.
    </bevon:description>
        <bevon:name xml:lang="en">Don Julio Blanco</bevon:name>
        <bevon:name xml:lang="ko">돈 훌리오 블랑코</bevon:name>
        <bevon:fermentation_base rdf:resource="http://dbpedia.org/resource/Agave"/>
        <bevon:manufacturer rdf:resource="http://dbpedia.org/resource/Diageo"/>
        <bevon:origin rdf:resource="http://dbpedia.org/resource/Mexico"/>
        <bevon:container rdf:resource="&bevon;container/750mlGlassBottle"/>
        <rdfs:seeAlso rdf:resource="http://www.donjulio.com/blanco.aspx"/>
        <bevon:color>
            <rdf:Description>
                <rdf:type rdf:resource="&dbpedia;Colour"/>
                <dcterms:title xml:lang="en">Clear</dcterms:title>
            </rdf:Description>
        </bevon:color>
    </owl:NamedIndividual>
    


    <!-- http://rdfs.co/bevon/beverage/Glenfiddich12YearOld -->

    <owl:NamedIndividual rdf:about="&bevon;beverage/Glenfiddich12YearOld">
        <rdf:type rdf:resource="&gr;ProductOrServiceModel"/>
        <rdf:type rdf:resource="&bevon;SpeysideSingleMalt"/>
        <bevon:launch rdf:datatype="&xsd;gYear">1887</bevon:launch>
        <bevon:abv rdf:datatype="&xsd;decimal">40</bevon:abv>
        <bevon:description xml:lang="en">
    Carefully matured in the finest American bourbon and Spanish sherry oak
    casks for at least 12 years. Married and mellowed in oak marrying tuns for
    complete harmony of aroma and flavor.

    A single malt Scotch whisky with distinctive fresh pear, creamy with subtle
    oak flavors and a long smooth and mellow finish.
    </bevon:description>
        <bevon:name xml:lang="en">Glenfiddich 12 Year Old</bevon:name>
        <bevon:name xml:lang="ko">글렌피딕 12년</bevon:name>
        <bevon:fermentation_base rdf:resource="http://dbpedia.org/resource/Barley"/>
        <bevon:origin rdf:resource="http://dbpedia.org/resource/Strathspey,_Scotland"/>
        <bevon:manufacturer rdf:resource="http://dbpedia.org/resource/William_Grant_%26_Sons"/>
        <bevon:container rdf:resource="&bevon;container/700mlGlassBottle"/>
        <bevon:aging>
            <rdf:Description>
                <rdf:type rdf:resource="&bevon;Aging"/>
                <bevon:previous_content rdf:resource="http://dbpedia.org/resource/Bourbon_whiskey"/>
                <bevon:material rdf:resource="http://dbpedia.org/resource/Oak"/>
                <bevon:previous_content rdf:resource="http://dbpedia.org/resource/Sherry"/>
                <bevon:duration>
                    <rdf:Description>
                        <rdf:type rdf:resource="&time;DurationDescription"/>
                    </rdf:Description>
                </bevon:duration>
            </rdf:Description>
        </bevon:aging>
        <bevon:distillery>
            <rdf:Description>
                <rdf:type rdf:resource="&bevon;Distillery"/>
                <whisky:region rdf:resource="http://dbpedia.org/resource/Strathspey,_Scotland"/>
                <whisky:owner rdf:resource="http://dbpedia.org/resource/William_Grant_%26_Sons"/>
                <whisky:waterSource>
                    <rdf:Description>
                        <rdf:type rdf:resource="&whisky;WaterSource"/>
                        <dcterms:title xml:lang="en">Robbie Dhu Springs</dcterms:title>
                        <dcterms:title xml:lang="ko">로비 듀 수원지</dcterms:title>
                    </rdf:Description>
                </whisky:waterSource>
            </rdf:Description>
        </bevon:distillery>
        <bevon:color>
            <rdf:Description>
                <rdf:type rdf:resource="&dbpedia;Colour"/>
                <dcterms:title xml:lang="en">Gold</dcterms:title>
            </rdf:Description>
        </bevon:color>
    </owl:NamedIndividual>
    


    <!-- http://rdfs.co/bevon/beverage/Guinness -->

    <owl:NamedIndividual rdf:about="&bevon;beverage/Guinness">
        <rdf:type rdf:resource="&gr;ProductOrServiceModel"/>
        <rdf:type rdf:resource="&bevon;DryStout"/>
        <bevon:launch rdf:datatype="&xsd;gYear">1759</bevon:launch>
        <bevon:srm rdf:datatype="&xsd;nonNegativeInteger">32</bevon:srm>
        <bevon:ibu rdf:datatype="&xsd;nonNegativeInteger">37</bevon:ibu>
        <bevon:abv rdf:datatype="&xsd;decimal">4.2</bevon:abv>
        <bevon:description xml:lang="en">
    Guinness is a popular Irish dry stout that originated in the brewery of
    Arthur Guinness (1725–1803) at St. James&apos;s Gate, Dublin. Guinness is one
    of the most successful beer brands worldwide.
    </bevon:description>
        <bevon:name xml:lang="en">Guinness Draught</bevon:name>
        <bevon:name xml:lang="ko">기네스 드래프트</bevon:name>
        <bevon:fermentation_base rdf:resource="http://dbpedia.org/resource/Barley"/>
        <bevon:manufacturer rdf:resource="http://dbpedia.org/resource/Diageo"/>
        <bevon:origin rdf:resource="http://dbpedia.org/resource/Dublin"/>
        <rdfs:seeAlso rdf:resource="http://en.wikipedia.org/wiki/Guinness"/>
        <bevon:container rdf:resource="&bevon;container/15lBeerKeg"/>
        <bevon:container rdf:resource="&bevon;container/30lBeerKeg"/>
        <bevon:container rdf:resource="&bevon;container/330mlBeverageCan"/>
        <bevon:container rdf:resource="&bevon;container/330mlLongneck"/>
    </owl:NamedIndividual>
    


    <!-- http://rdfs.co/bevon/beverage/Kilkenny -->

    <owl:NamedIndividual rdf:about="&bevon;beverage/Kilkenny">
        <rdf:type rdf:resource="&gr;ProductOrServiceModel"/>
        <rdf:type rdf:resource="&bevon;IrishRedAle"/>
        <bevon:srm rdf:datatype="&xsd;nonNegativeInteger">14</bevon:srm>
        <bevon:launch rdf:datatype="&xsd;gYear">1710</bevon:launch>
        <bevon:ibu rdf:datatype="&xsd;nonNegativeInteger">23</bevon:ibu>
        <bevon:abv rdf:datatype="&xsd;decimal">4.3</bevon:abv>
        <bevon:description xml:lang="en">
    Kilkenny is a nitrogenated Irish cream ale from the makers of Guinness,
    which originated in Kilkenny, Ireland. The brand is managed and produced
    by Diageo. It is available in draught and cans. It is brewed in Ireland
    and its heritage dates back to the 14th century.
    </bevon:description>
        <bevon:name xml:lang="en">Kilkenny Irish Cream Ale</bevon:name>
        <bevon:name xml:lang="ko">킬케니 아이리쉬 크림 에일</bevon:name>
        <bevon:fermentation_base rdf:resource="http://dbpedia.org/resource/Barley"/>
        <bevon:manufacturer rdf:resource="http://dbpedia.org/resource/Diageo"/>
        <bevon:origin rdf:resource="http://dbpedia.org/resource/Kilkenny"/>
        <rdfs:seeAlso rdf:resource="http://en.wikipedia.org/wiki/Kilkenny_(beer)"/>
        <bevon:similar rdf:resource="&bevon;beverage/Smithwicks"/>
        <bevon:container rdf:resource="&bevon;container/30lBeerKeg"/>
        <bevon:container rdf:resource="&bevon;container/440mlBeverageCan"/>
    </owl:NamedIndividual>
    


    <!-- http://rdfs.co/bevon/beverage/KozelDark -->

    <owl:NamedIndividual rdf:about="&bevon;beverage/KozelDark">
        <rdf:type rdf:resource="&gr;ProductOrServiceModel"/>
        <rdf:type rdf:resource="&bevon;Dunkel"/>
        <bevon:launch rdf:datatype="&xsd;gYear">1874</bevon:launch>
        <bevon:abv rdf:datatype="&xsd;decimal">3.8</bevon:abv>
        <bevon:name xml:lang="cs">Velkopopovický Kozel Černý</bevon:name>
        <bevon:description xml:lang="en">
    Velkopopovický Kozel Dark beer is brewed to the original recipe using a
    special mix of dark malts, clean water from our own well close to the
    brewery, and a selection of the best hops. The caramelized malt gives this
    beer a unique ruby color and sweet flavor, thanks to which it is
    appreciated and respected all over the world.
    </bevon:description>
        <bevon:name xml:lang="en">Velkopopovický Kozel Dark</bevon:name>
        <bevon:name xml:lang="ko">코젤 다크</bevon:name>
        <bevon:fermentation_base rdf:resource="http://dbpedia.org/resource/Barley"/>
        <bevon:manufacturer rdf:resource="http://dbpedia.org/resource/SABMiller"/>
        <bevon:origin rdf:resource="http://dbpedia.org/resource/Velké_Popovice"/>
        <bevon:container rdf:resource="&bevon;container/500mlLongneck"/>
    </owl:NamedIndividual>
    


    <!-- http://rdfs.co/bevon/beverage/Smithwicks -->

    <owl:NamedIndividual rdf:about="&bevon;beverage/Smithwicks">
        <rdf:type rdf:resource="&gr;ProductOrServiceModel"/>
        <rdf:type rdf:resource="&bevon;IrishRedAle"/>
        <bevon:srm rdf:datatype="&xsd;nonNegativeInteger">14</bevon:srm>
        <bevon:launch rdf:datatype="&xsd;gYear">1710</bevon:launch>
        <bevon:ibu rdf:datatype="&xsd;nonNegativeInteger">20</bevon:ibu>
        <bevon:abv rdf:datatype="&xsd;decimal">3.8</bevon:abv>
        <bevon:description xml:lang="en">
    Smithwick&apos;s is an Irish red ale style beer from Kilkenny, Ireland. It is a
    clear beer with a rich ruby color and creamy head.
    </bevon:description>
        <bevon:name xml:lang="en">Smithwick&apos;s Superior Irish Ale</bevon:name>
        <bevon:name xml:lang="ko">스미딕스 슈페리어 아이리쉬 에일</bevon:name>
        <bevon:fermentation_base rdf:resource="http://dbpedia.org/resource/Barley"/>
        <bevon:manufacturer rdf:resource="http://dbpedia.org/resource/Diageo"/>
        <bevon:origin rdf:resource="http://dbpedia.org/resource/Kilkenny"/>
        <rdfs:seeAlso rdf:resource="http://en.wikipedia.org/wiki/Smithwick%27s"/>
        <bevon:similar rdf:resource="&bevon;beverage/Kilkenny"/>
        <bevon:container rdf:resource="&bevon;container/30lBeerKeg"/>
        <bevon:container rdf:resource="&bevon;container/330mlLongneck"/>
        <bevon:container rdf:resource="&bevon;container/440mlBeverageCan"/>
        <bevon:color>
            <rdf:Description>
                <rdf:type rdf:resource="&dbpedia;Colour"/>
                <dcterms:title xml:lang="en">Ruby Red</dcterms:title>
            </rdf:Description>
        </bevon:color>
    </owl:NamedIndividual>
    


    <!-- http://rdfs.co/bevon/beverage/Tsingtao -->

    <owl:NamedIndividual rdf:about="&bevon;beverage/Tsingtao">
        <rdf:type rdf:resource="&gr;ProductOrServiceModel"/>
        <rdf:type rdf:resource="&bevon;Pilsner"/>
        <bevon:launch rdf:datatype="&xsd;gYear">1904</bevon:launch>
        <bevon:ibu rdf:datatype="&xsd;nonNegativeInteger">20</bevon:ibu>
        <bevon:srm rdf:datatype="&xsd;nonNegativeInteger">4</bevon:srm>
        <bevon:abv rdf:datatype="&xsd;decimal">4.7</bevon:abv>
        <bevon:description xml:lang="en">
    Tsingtao Lager, a well-hopped standard pilsner of 4.7% alcohol, is the
    flagship brew, accounting for most of the brewery&apos;s production.
    </bevon:description>
        <bevon:name xml:lang="en">Tsingtao Lager</bevon:name>
        <bevon:name xml:lang="ko">칭타오 라거</bevon:name>
        <bevon:fermentation_base rdf:resource="http://dbpedia.org/resource/Barley"/>
        <bevon:origin rdf:resource="http://dbpedia.org/resource/Qingdao"/>
        <bevon:manufacturer rdf:resource="http://dbpedia.org/resource/Tsingtao_Brewery"/>
        <bevon:brewery rdf:resource="http://dbpedia.org/resource/Tsingtao_Brewery"/>
        <bevon:container rdf:resource="&bevon;container/330mlLongneck"/>
        <bevon:container rdf:resource="&bevon;container/355mlBeverageCan"/>
        <bevon:container rdf:resource="&bevon;container/500mlBeverageCan"/>
        <bevon:container rdf:resource="&bevon;container/640mlLongneck"/>
    </owl:NamedIndividual>
    


    <!-- http://rdfs.co/bevon/beverage/WhiskyAndSoda -->

    <owl:NamedIndividual rdf:about="&bevon;beverage/WhiskyAndSoda">
        <rdf:type rdf:resource="&gr;ProductOrServiceModel"/>
        <rdf:type rdf:resource="&bevon;Highball"/>
        <bevon:description xml:lang="en">
    Whisky &amp; Soda is a kind of mixed drinks that are composed of whisky and
    carbonated water.
    </bevon:description>
        <bevon:name xml:lang="en">Whisky &amp; Soda</bevon:name>
        <bevon:name xml:lang="ko">위스키 소다</bevon:name>
        <bevon:ingredient>
            <rdf:Description>
                <rdf:type rdf:resource="&food;Ingredient"/>
                <bevon:food>
                    <rdf:Description>
                        <rdf:type rdf:resource="&bevon;CarbonatedWater"/>
                        <dcterms:title xml:lang="en">Carbonated Water</dcterms:title>
                    </rdf:Description>
                </bevon:food>
            </rdf:Description>
        </bevon:ingredient>
        <bevon:ingredient>
            <rdf:Description>
                <rdf:type rdf:resource="&food;Ingredient"/>
                <bevon:food>
                    <rdf:Description>
                        <rdf:type rdf:resource="&bevon;Whisky"/>
                        <dcterms:title xml:lang="en">Whisky</dcterms:title>
                    </rdf:Description>
                </bevon:food>
                <bevon:quantity>
                    <rdf:Description>
                        <rdf:type rdf:resource="&gr;QuantitativeValueInteger"/>
                    </rdf:Description>
                </bevon:quantity>
            </rdf:Description>
        </bevon:ingredient>
    </owl:NamedIndividual>
    


    <!-- http://rdfs.co/bevon/container/1_8lPlasticBottle -->

    <owl:NamedIndividual rdf:about="&bevon;container/1_8lPlasticBottle">
        <rdf:type rdf:resource="&bevon;PlasticBottle"/>
        <skos:prefLabel xml:lang="en">1.8l Plastic Bottle</skos:prefLabel>
        <skos:prefLabel xml:lang="ko">1.8l 플라스틱 병</skos:prefLabel>
        <bevon:volume>
            <rdf:Description>
                <rdf:type rdf:resource="&gr;QuantitativeValueFloat"/>
            </rdf:Description>
        </bevon:volume>
    </owl:NamedIndividual>
    


    <!-- http://rdfs.co/bevon/container/15lBeerKeg -->

    <owl:NamedIndividual rdf:about="&bevon;container/15lBeerKeg">
        <rdf:type rdf:resource="&bevon;BeerKeg"/>
        <skos:prefLabel xml:lang="en">15l Beer Keg</skos:prefLabel>
        <skos:prefLabel xml:lang="ko">15l 맥주 케그</skos:prefLabel>
        <bevon:volume>
            <rdf:Description>
                <rdf:type rdf:resource="&gr;QuantitativeValueInteger"/>
            </rdf:Description>
        </bevon:volume>
    </owl:NamedIndividual>
    


    <!-- http://rdfs.co/bevon/container/200mlPlasticBottle -->

    <owl:NamedIndividual rdf:about="&bevon;container/200mlPlasticBottle">
        <rdf:type rdf:resource="&bevon;PlasticBottle"/>
        <skos:prefLabel xml:lang="en">200ml Plastic Bottle</skos:prefLabel>
        <skos:prefLabel xml:lang="ko">200ml 플라스틱 병</skos:prefLabel>
        <bevon:volume>
            <rdf:Description>
                <rdf:type rdf:resource="&gr;QuantitativeValueInteger"/>
            </rdf:Description>
        </bevon:volume>
    </owl:NamedIndividual>
    


    <!-- http://rdfs.co/bevon/container/25lBeerKeg -->

    <owl:NamedIndividual rdf:about="&bevon;container/25lBeerKeg">
        <rdf:type rdf:resource="&bevon;BeerKeg"/>
        <skos:prefLabel xml:lang="en">25l Beer Keg</skos:prefLabel>
        <skos:prefLabel xml:lang="ko">25l 맥주 케그</skos:prefLabel>
        <bevon:volume>
            <rdf:Description>
                <rdf:type rdf:resource="&gr;QuantitativeValueInteger"/>
            </rdf:Description>
        </bevon:volume>
    </owl:NamedIndividual>
    


    <!-- http://rdfs.co/bevon/container/30lBeerKeg -->

    <owl:NamedIndividual rdf:about="&bevon;container/30lBeerKeg">
        <rdf:type rdf:resource="&bevon;BeerKeg"/>
        <skos:prefLabel xml:lang="en">30l Beer Keg</skos:prefLabel>
        <skos:prefLabel xml:lang="ko">30l 맥주 케그</skos:prefLabel>
        <bevon:volume>
            <rdf:Description>
                <rdf:type rdf:resource="&gr;QuantitativeValueInteger"/>
            </rdf:Description>
        </bevon:volume>
    </owl:NamedIndividual>
    


    <!-- http://rdfs.co/bevon/container/330mlBeverageCan -->

    <owl:NamedIndividual rdf:about="&bevon;container/330mlBeverageCan">
        <rdf:type rdf:resource="&bevon;BeverageCan"/>
        <skos:prefLabel xml:lang="en">330ml Beverage Can</skos:prefLabel>
        <skos:prefLabel xml:lang="ko">330ml 음료 캔</skos:prefLabel>
        <bevon:volume>
            <rdf:Description>
                <rdf:type rdf:resource="&gr;QuantitativeValueInteger"/>
            </rdf:Description>
        </bevon:volume>
    </owl:NamedIndividual>
    


    <!-- http://rdfs.co/bevon/container/330mlLongneck -->

    <owl:NamedIndividual rdf:about="&bevon;container/330mlLongneck">
        <rdf:type rdf:resource="&bevon;Longneck"/>
        <skos:prefLabel xml:lang="en">330ml Longneck Bottle</skos:prefLabel>
        <skos:prefLabel xml:lang="ko">330ml 긴목 맥주병</skos:prefLabel>
        <bevon:volume>
            <rdf:Description>
                <rdf:type rdf:resource="&gr;QuantitativeValueInteger"/>
            </rdf:Description>
        </bevon:volume>
    </owl:NamedIndividual>
    


    <!-- http://rdfs.co/bevon/container/355mlBeverageCan -->

    <owl:NamedIndividual rdf:about="&bevon;container/355mlBeverageCan">
        <rdf:type rdf:resource="&bevon;BeverageCan"/>
        <skos:prefLabel xml:lang="en">355ml Beverage Can</skos:prefLabel>
        <skos:prefLabel xml:lang="ko">355ml 음료 캔</skos:prefLabel>
        <bevon:volume>
            <rdf:Description>
                <rdf:type rdf:resource="&gr;QuantitativeValueInteger"/>
            </rdf:Description>
        </bevon:volume>
    </owl:NamedIndividual>
    


    <!-- http://rdfs.co/bevon/container/360mlGlassBottle -->

    <owl:NamedIndividual rdf:about="&bevon;container/360mlGlassBottle">
        <rdf:type rdf:resource="&bevon;GlassBottle"/>
        <skos:prefLabel xml:lang="en">360ml Glass Bottle</skos:prefLabel>
        <skos:prefLabel xml:lang="ko">360ml 유리병</skos:prefLabel>
        <bevon:volume>
            <rdf:Description>
                <rdf:type rdf:resource="&gr;QuantitativeValueInteger"/>
            </rdf:Description>
        </bevon:volume>
    </owl:NamedIndividual>
    


    <!-- http://rdfs.co/bevon/container/360mlPlasticBottle -->

    <owl:NamedIndividual rdf:about="&bevon;container/360mlPlasticBottle">
        <rdf:type rdf:resource="&bevon;PlasticBottle"/>
        <skos:prefLabel xml:lang="en">360ml Plastic Bottle</skos:prefLabel>
        <skos:prefLabel xml:lang="ko">360ml 플라스틱 병</skos:prefLabel>
        <bevon:volume>
            <rdf:Description>
                <rdf:type rdf:resource="&gr;QuantitativeValueInteger"/>
            </rdf:Description>
        </bevon:volume>
    </owl:NamedIndividual>
    


    <!-- http://rdfs.co/bevon/container/440mlBeverageCan -->

    <owl:NamedIndividual rdf:about="&bevon;container/440mlBeverageCan">
        <rdf:type rdf:resource="&bevon;BeverageCan"/>
        <skos:prefLabel xml:lang="en">440ml Beverage Can</skos:prefLabel>
        <skos:prefLabel xml:lang="ko">440ml 음료 캔</skos:prefLabel>
        <bevon:volume>
            <rdf:Description>
                <rdf:type rdf:resource="&gr;QuantitativeValueInteger"/>
            </rdf:Description>
        </bevon:volume>
    </owl:NamedIndividual>
    


    <!-- http://rdfs.co/bevon/container/50lBeerKeg -->

    <owl:NamedIndividual rdf:about="&bevon;container/50lBeerKeg">
        <rdf:type rdf:resource="&bevon;BeerKeg"/>
        <skos:prefLabel xml:lang="en">50l Beer Keg</skos:prefLabel>
        <skos:prefLabel xml:lang="ko">50l 맥주 케그</skos:prefLabel>
        <bevon:volume>
            <rdf:Description>
                <rdf:type rdf:resource="&gr;QuantitativeValueInteger"/>
            </rdf:Description>
        </bevon:volume>
    </owl:NamedIndividual>
    


    <!-- http://rdfs.co/bevon/container/500mlBeverageCan -->

    <owl:NamedIndividual rdf:about="&bevon;container/500mlBeverageCan">
        <rdf:type rdf:resource="&bevon;BeverageCan"/>
        <skos:prefLabel xml:lang="en">500ml Beverage Can</skos:prefLabel>
        <skos:prefLabel xml:lang="ko">500ml 음료 캔</skos:prefLabel>
        <bevon:volume>
            <rdf:Description>
                <rdf:type rdf:resource="&gr;QuantitativeValueInteger"/>
            </rdf:Description>
        </bevon:volume>
    </owl:NamedIndividual>
    


    <!-- http://rdfs.co/bevon/container/500mlLongneck -->

    <owl:NamedIndividual rdf:about="&bevon;container/500mlLongneck">
        <rdf:type rdf:resource="&bevon;Longneck"/>
        <skos:prefLabel xml:lang="en">500ml Longneck Bottle</skos:prefLabel>
        <skos:prefLabel xml:lang="ko">500ml 긴목 맥주병</skos:prefLabel>
        <bevon:volume>
            <rdf:Description>
                <rdf:type rdf:resource="&gr;QuantitativeValueInteger"/>
            </rdf:Description>
        </bevon:volume>
    </owl:NamedIndividual>
    


    <!-- http://rdfs.co/bevon/container/640mlLongneck -->

    <owl:NamedIndividual rdf:about="&bevon;container/640mlLongneck">
        <rdf:type rdf:resource="&bevon;Longneck"/>
        <skos:prefLabel xml:lang="en">640ml Longneck Bottle</skos:prefLabel>
        <skos:prefLabel xml:lang="ko">640ml 긴목 맥주병</skos:prefLabel>
        <bevon:volume>
            <rdf:Description>
                <rdf:type rdf:resource="&gr;QuantitativeValueInteger"/>
            </rdf:Description>
        </bevon:volume>
    </owl:NamedIndividual>
    


    <!-- http://rdfs.co/bevon/container/640mlPlasticBottle -->

    <owl:NamedIndividual rdf:about="&bevon;container/640mlPlasticBottle">
        <rdf:type rdf:resource="&bevon;PlasticBottle"/>
        <skos:prefLabel xml:lang="en">640ml Plastic Bottle</skos:prefLabel>
        <skos:prefLabel xml:lang="ko">640ml 플라스틱 병</skos:prefLabel>
        <bevon:volume>
            <rdf:Description>
                <rdf:type rdf:resource="&gr;QuantitativeValueInteger"/>
            </rdf:Description>
        </bevon:volume>
    </owl:NamedIndividual>
    


    <!-- http://rdfs.co/bevon/container/700mlGlassBottle -->

    <owl:NamedIndividual rdf:about="&bevon;container/700mlGlassBottle">
        <rdf:type rdf:resource="&bevon;GlassBottle"/>
        <skos:prefLabel xml:lang="en">700ml Glass Bottle</skos:prefLabel>
        <skos:altLabel xml:lang="en">70cl Glass Bottle</skos:altLabel>
        <skos:prefLabel xml:lang="ko">700ml 유리병</skos:prefLabel>
        <bevon:volume>
            <rdf:Description>
                <rdf:type rdf:resource="&gr;QuantitativeValueInteger"/>
            </rdf:Description>
        </bevon:volume>
    </owl:NamedIndividual>
    


    <!-- http://rdfs.co/bevon/container/750mlGlassBottle -->

    <owl:NamedIndividual rdf:about="&bevon;container/750mlGlassBottle">
        <rdf:type rdf:resource="&bevon;GlassBottle"/>
        <skos:prefLabel xml:lang="en">750ml Glass Bottle</skos:prefLabel>
        <skos:altLabel xml:lang="en">75cl Glass Bottle</skos:altLabel>
        <skos:prefLabel xml:lang="ko">750ml 유리병</skos:prefLabel>
        <bevon:volume>
            <rdf:Description>
                <rdf:type rdf:resource="&gr;QuantitativeValueInteger"/>
            </rdf:Description>
        </bevon:volume>
    </owl:NamedIndividual>
    


    <!-- http://www.w3.org/TR/2003/PR-owl-guide-20031209/wine#RedWine -->

    <owl:NamedIndividual rdf:about="&wine;RedWine"/>
    


    <!-- http://www.w3.org/TR/2003/PR-owl-guide-20031209/wine#WhiteWine -->

    <owl:NamedIndividual rdf:about="&wine;WhiteWine"/>
    <rdf:Description>
        <dcterms:creator rdf:resource="http://jayg.me/"/>
    </rdf:Description>
    <rdf:Description>
        <rdfs:label xml:lang="en">Whisky &amp; Soda</rdfs:label>
        <rdfs:comment rdf:datatype="&rdf;XMLLiteral">
    &lt;pre&gt;&lt;code&gt;beverage:WhiskyAndSoda
  a owl:NamedIndividual, bevon:Highball , gr:ProductOrServiceModel ;
  bevon:name &quot;Whisky &amp;amp; Soda&quot;@en , &quot;위스키 소다&quot;@ko ;
  bevon:description &quot;&quot;&quot;
    Whisky &amp;amp; Soda is a kind of mixed drinks that are composed of whisky and
    carbonated water.
    &quot;&quot;&quot;@en ;
  bevon:ingredient [
    a food:Ingredient ;
    bevon:food [
      a bevon:Whisky ;
      owl:sameAs &amp;lt;http://dbpedia.org/resource/Whisky&amp;gt; ;
      dcterms:title &quot;Whisky&quot;@en
    ] ;
    bevon:quantity [
      a gr:QuantitativeValueInteger ;
      gr:hasUnitOfMeasurement &quot;OZA&quot; ;
      gr:hasValue &quot;2&quot;^^xsd:int
    ]
  ] , [
    a food:Ingredient ;
    bevon:food [
      a bevon:CarbonatedWater ;
      owl:sameAs &amp;lt;http://dbpedia.org/resource/Carbonated_water&amp;gt; ;
      dcterms:title &quot;Carbonated Water&quot;@en
    ]
  ] .&lt;/code&gt;&lt;/pre&gt;
    </rdfs:comment>
    </rdf:Description>
    <rdf:Description>
        <rdfs:label xml:lang="en">Glenfiddich 12 Year Old</rdfs:label>
        <rdfs:comment rdf:datatype="&rdf;XMLLiteral">
    &lt;pre&gt;&lt;code&gt;beverage:Glenfiddich12YearOld
  a owl:NamedIndividual, bevon:SpeysideSingleMalt , gr:ProductOrServiceModel ;
  bevon:name &quot;Glenfiddich 12 Year Old&quot;@en , &quot;글렌피딕 12년&quot;@ko ;
  bevon:description &quot;&quot;&quot;
    Carefully matured in the finest American bourbon and Spanish sherry oak
    casks for at least 12 years. Married and mellowed in oak marrying tuns for
    complete harmony of aroma and flavor.

    A single malt Scotch whisky with distinctive fresh pear, creamy with subtle
    oak flavors and a long smooth and mellow finish.
    &quot;&quot;&quot;@en ;
  bevon:origin &amp;lt;http://dbpedia.org/resource/Strathspey,_Scotland&amp;gt; ;
  bevon:launch &quot;1887&quot;^^xsd:gYear ;
  bevon:distillery [
    a bevon:Distillery ;
    owl:sameAs &amp;lt;http://dbpedia.org/resource/Glenfiddich_distillery&amp;gt; ;
    whisky:region &amp;lt;http://dbpedia.org/resource/Strathspey,_Scotland&amp;gt; ;
    whisky:owner &amp;lt;http://dbpedia.org/resource/William_Grant_%26_Sons&amp;gt; ;
    whisky:waterSource [
      a whisky:WaterSource ;
      dcterms:title &quot;Robbie Dhu Springs&quot;@en , &quot;로비 듀 수원지&quot;@ko
    ]
  ] ;
  bevon:manufacturer &amp;lt;http://dbpedia.org/resource/William_Grant_%26_Sons&amp;gt; ;
  bevon:fermentation_base &amp;lt;http://dbpedia.org/resource/Barley&amp;gt; ;
  bevon:aging [
    a bevon:Aging ;
    bevon:material &amp;lt;http://dbpedia.org/resource/Oak&amp;gt; ;
    bevon:previous_content
      &amp;lt;http://dbpedia.org/resource/Bourbon_whiskey&amp;gt; ,
      &amp;lt;http://dbpedia.org/resource/Sherry&amp;gt; ;
    bevon:duration [
      a time:DurationDescription ;
      time:years &quot;12&quot;^^xsd:decimal
    ]
  ] ;
  bevon:color [
    a dbpedia:Colour ;
    owl:sameAs &amp;lt;http://dbpedia.org/resource/Gold_(color)&amp;gt; ;
    owl:sameAs &amp;lt;http://purl.org/colors/rgb/FFD700&amp;gt; ;
    dcterms:title &quot;Gold&quot;@en
  ] ;
  bevon:abv &quot;40&quot;^^xsd:decimal ;
  bevon:container container:700mlGlassBottle .

container:700mlGlassBottle a owl:NamedIndividual, bevon:GlassBottle ;
  skos:prefLabel &quot;700ml Glass Bottle&quot;@en , &quot;700ml 유리병&quot;@ko ;
  skos:altLabel &quot;70cl Glass Bottle&quot;@en ;
  bevon:volume [
    a gr:QuantitativeValueInteger ;
    gr:hasUnitOfMeasurement &quot;MLT&quot; ;
    gr:hasValue &quot;700&quot;^^xsd:int
  ] .&lt;/code&gt;&lt;/pre&gt;
    </rdfs:comment>
    </rdf:Description>
    <rdf:Description>
        <dcterms:creator rdf:resource="http://jayg.me/"/>
    </rdf:Description>
    <rdf:Description>
        <dcterms:creator rdf:resource="http://jayg.me/"/>
    </rdf:Description>
    <rdf:Description>
        <dcterms:creator rdf:resource="http://jayg.me/"/>
    </rdf:Description>
    <rdf:Description>
        <dcterms:creator rdf:resource="http://jayg.me/"/>
    </rdf:Description>
    <rdf:Description>
        <dcterms:creator rdf:resource="http://jayg.me/"/>
    </rdf:Description>
    


    <!-- 
    ///////////////////////////////////////////////////////////////////////////////////////
    //
    // Annotations
    //
    ///////////////////////////////////////////////////////////////////////////////////////
     -->

    <rdf:Description rdf:about="&bevon;0.7/html">
        <dcterms:format>
            <rdf:Description>
                <rdf:type rdf:resource="&dcterms;IMT"/>
                <rdfs:label xml:lang="en">HTML</rdfs:label>
            </rdf:Description>
        </dcterms:format>
    </rdf:Description>
    <rdf:Description rdf:about="&bevon;0.7/rdf">
        <dcterms:format>
            <rdf:Description>
                <rdf:type rdf:resource="&dcterms;IMT"/>
                <rdfs:label xml:lang="en">RDF/XML</rdfs:label>
            </rdf:Description>
        </dcterms:format>
    </rdf:Description>
    <rdf:Description rdf:about="&bevon;0.7/ttl">
        <dcterms:format>
            <rdf:Description>
                <rdf:type rdf:resource="&dcterms;IMT"/>
                <rdfs:label xml:lang="en">Turtle</rdfs:label>
            </rdf:Description>
        </dcterms:format>
    </rdf:Description>
</rdf:RDF>



<!-- Generated by the OWL API (version 3.5.0) http://owlapi.sourceforge.net -->

